Introduce Class level generics
* Introducing class level generics

Update the language to support class level generics.
The most notable other additions are correctness predicates, to ensure type substitution are always valid.

We make interp_class more precise, asserting that all
fields must be in their interpretation at the "dynamic" type,
not at the static type (where we only know some of them).
We can still derive the part about static type if necessary (see
interp_fields_is_inclusion)

theories/examples.v
@@ -13,48 +13,73 @@ From iris.algebra.lib Require Import gmap_view.
 From shack Require Import lang heap modality interp adequacy.
 
 (* TODO: we don't have void atm so I'm using null ;) *)
-(* Definition of class BoxInt:
- * class BoxInt {
- *   int $data;
- *   function set(int $data) : void { $this->data = $data; }
- *   function get(): int { $ret = $this->data; return $ret; }
+
+(* Definition of class Box<T>:
+ * class Box<T> {
+ *   T $data;
+ *   function set(T $data) : void { $this->data = $data; }
+ *   function get(): T { $ret = $this->data; return $ret; }
  * }
  *)
-Definition BoxIntSet := {|
+Definition BoxSet := {|
   methodname := "set";
-  methodargs := {["$data" := IntT ]};
+  methodargs := {["$data" := GenT 0 ]};
   methodrettype := NullT;
   methodbody := SetC (VarE "$this") "$data" (VarE "$data");
   methodret := NullE;
 |}.
 
-Definition BoxIntGet := {|
+Definition BoxGet := {|
   methodname := "get";
   methodargs := ∅;
-  methodrettype := IntT;
+  methodrettype := GenT 0;
   methodbody := GetC "$ret" (VarE "$this") "$data";
   methodret := VarE "$ret";
 |}.
 
-Definition BoxInt := {|
-  classname := "BoxInt";
+Definition Box := {|
+  classname := "Box";
   superclass := None;
-  classfields := {["$data" := IntT]};
-  classmethods := <["set" := BoxIntSet]>{["get" := BoxIntGet]};
+  generics := 1;
+  classfields := {["$data" := GenT 0]};
+  classmethods := {["set" := BoxSet; "get" := BoxGet]};
+|}.
+
+(* Definition of class IntBoxS:
+ * class IntBoxS extends Box<int> {
+ * function set(int $data) : void { $this->data = $data + 1; }
+ *)
+
+Definition σ : list lang_ty := [IntT].
+
+Definition IntBoxSSet := {|
+  methodname := "set";
+  methodargs := {["$data" := IntT ]};
+  methodrettype := NullT;
+  methodbody := SetC (VarE "$this") "$data" (OpE PlusO (VarE "$data") (IntE 1%Z));
+  methodret := NullE;
+|}.
+
+Definition IntBoxS := {|
+  classname := "IntBoxS";
+  superclass := Some ("Box", σ);
+  generics := 0;
+  classfields := ∅;
+  classmethods := {["set" := IntBoxSSet]};
 |}.
 
 (* Main program:
  * function main(): bool {
- *   $box = new BoxInt(32);
+ *   $box = new IntBoxS(32);
  *   $tmp = $box->get();
  *   $tmp = $tmp + 20;
  *   $_ = $box->set($tmp - 10);
  *   $tmp = $box->data;
- *   return ($tmp == 42);
+ *   return ($tmp == 43);
  * }
  *)
 Definition ProgramBody :=
-   SeqC (NewC "$box" "BoxInt" {["$data" := IntE 32]})
+   SeqC (NewC "$box" "IntBoxS" {["$data" := IntE 32]})
   (SeqC (CallC "$tmp" (VarE "$box") "get" ∅)
   (SeqC (LetC "$tmp" (OpE PlusO (VarE "$tmp") (IntE 20)))
   (SeqC (CallC "$_" (VarE "$box") "set"
@@ -67,36 +92,67 @@ Definition Main := {|
   methodargs := ∅;
   methodrettype := BoolT;
   methodbody := ProgramBody;
-  methodret := OpE EqO (VarE "$tmp") (IntE 42);
+  methodret := OpE EqO (VarE "$tmp") (IntE 43);
 |}.
 
-Local Instance PDC : ProgDefContext := { Δ := {[ "BoxInt" := BoxInt ]} }.
+Local Instance PDC : ProgDefContext := { Δ := {[ "Box" := Box; "IntBoxS" := IntBoxS ]} }.
 
-Lemma has_method_get: has_method "get" BoxIntGet "BoxInt".
+Lemma wfσ : Forall wf_ty σ.
+Proof.
+  apply Forall_forall => x hx.
+  apply elem_of_list_lookup_1 in hx.
+  destruct hx as [n hx].
+  rewrite /σ /= in hx.
+  apply list_lookup_singleton_Some in hx as [-> <-].
+  by constructor.
+Qed.
+
+Lemma σbounded : Forall (bounded (generics IntBoxS)) σ.
+Proof.
+  apply Forall_forall => x hx.
+  apply elem_of_list_lookup_1 in hx.
+  destruct hx as [n hx].
+  rewrite /σ /= in hx.
+  apply list_lookup_singleton_Some in hx as [-> <-].
+  by constructor.
+Qed.
+
+Lemma has_method_get: has_method "get" "IntBoxS" "Box" (subst_mdef σ BoxGet).
 Proof. by repeat econstructor; eauto. Qed.
 
-Lemma has_method_set: has_method "set" BoxIntSet "BoxInt".
+Lemma has_method_set: has_method "set" "IntBoxS" "IntBoxS" IntBoxSSet.
 Proof. by repeat econstructor; eauto. Qed.
 
-Lemma has_fields_BoxInt : has_fields "BoxInt" {[ "$data" := IntT ]}.
+Lemma has_fields_IntBoxS : has_fields "IntBoxS" {[ "$data" := IntT ]}.
 Proof.
   move => f fty; split => h.
   - inv h.
-    + rewrite /Δ /= lookup_insert in H; simplify_eq.
-      by rewrite /BoxInt /= in H0.
-    + rewrite /Δ /= lookup_insert in H; by simplify_eq.
+    + rewrite /Δ /= lookup_insert_ne // lookup_insert in H; by simplify_eq.
+    + rewrite /Δ /= lookup_insert_ne // lookup_insert in H; simplify_eq.
+      rewrite /IntBoxS /= in H1 H0.
+      injection H1; intros; subst; clear H1.
+      inv H2.
+      * rewrite /Δ /= lookup_insert in H; simplify_eq.
+        rewrite /Box /= lookup_insert_Some in H1.
+        destruct H1 as [[<- <-]|[?]]; last by rewrite lookup_empty in H1.
+        by rewrite lookup_insert.
+      * by rewrite /Δ /= lookup_insert in H; simplify_eq.
   - rewrite lookup_insert_Some in h.
-    destruct h as [[<- <-] | [? ?]]; first by eauto.
-    by rewrite lookup_empty in H0.
+    destruct h as [[<- <-] | [? h]]; last by rewrite lookup_empty in h.
+    change IntT with (subst_ty σ (GenT 0)).
+    eapply InheritsField => //.
+    econstructor.
+    + by rewrite /Δ /= lookup_insert.
+    + by rewrite /Box /=.
 Qed.
 
 Definition final_le le new_loc : local_env :=
    <["$_":=NullV]>
-  (<["$tmp":=IntV 42]>
+  (<["$tmp":=IntV 43]>
   (<["$box":=LocV new_loc]> le)).
 
 Definition final_heap (h: heap) new_loc :=
-  <[new_loc := ("BoxInt", {["$data" := IntV 42]})]> h.
+  <[new_loc := ("IntBoxS", {["$data" := IntV 43]})]> h.
 
 Lemma Main_eval st:
  ∀ new_loc, st.2 !! new_loc = None →
@@ -106,7 +162,7 @@ Proof.
   rewrite /ProgramBody.
   change 5 with (1 + (2 + (0 + (1 + 1)))).
   apply SeqEv with (<["$box" := LocV new_loc]>le,
-                    <[new_loc := ("BoxInt", {["$data" := IntV 32]})]> h).
+                    <[new_loc := ("IntBoxS", {["$data" := IntV 32]})]> h).
   { apply NewEv; first done.
     rewrite /map_args option_guard_True /=; first by rewrite omap_singleton.
     by apply map_Forall_singleton.
@@ -123,7 +179,7 @@ Proof.
       + by rewrite /= lookup_insert.
       + by rewrite lookup_insert.
       + by rewrite lookup_insert.
-    - by rewrite /BoxIntGet /= lookup_insert.
+    - by rewrite /BoxGet /= lookup_insert.
   }
   eapply SeqEv.
   { (* Let *)
@@ -140,16 +196,16 @@ Proof.
     - by rewrite lookup_insert.
     - by apply has_method_set.
     - by rewrite omap_singleton /= lookup_insert.
-    - rewrite /BoxIntSet /=.
+    - rewrite /IntBoxSSet /=.
       eapply SetEv.
       + by rewrite /= lookup_insert.
       + by rewrite /= lookup_insert_ne.
       + by rewrite lookup_insert.
       + done.
-    - by rewrite /BoxIntSet /=.
+    - by rewrite /IntBoxSSet /=.
   }
   replace (final_le le new_loc) with
-    ( <["$tmp" := IntV 42]>
+    ( <["$tmp" := IntV 43]>
      (<["$_":=NullV]>
      (<["$tmp":=IntV (32 + 20)]>
      (<["$tmp":=IntV 32]> (<["$box":=LocV new_loc]> le))))); last first.
@@ -165,8 +221,8 @@ Proof.
     by rewrite lookup_insert.
   }
   replace (final_heap h new_loc) with
-    ( <[new_loc:=("BoxInt", {["$data" := IntV (32 + 20 - 10); "$data" := IntV 32]})]>
-     (<[new_loc:=("BoxInt", {["$data" := IntV 32]})]> h)); last first.
+    ( <[new_loc:=("IntBoxS", {["$data" := IntV (33 + 20 - 10); "$data" := IntV 32]})]>
+     (<[new_loc:=("IntBoxS", {["$data" := IntV 32]})]> h)); last first.
   { rewrite /final_heap.
     apply map_eq => k.
     destruct (decide (k = new_loc)) as [-> | hne].
@@ -187,15 +243,16 @@ Qed.
 Definition final_lty lty : local_tys :=
    <["$tmp":=IntT]>
   (<["$_" := NullT]>
-  (<["$box":=ClassT "BoxInt"]> lty)).
+  (<["$box":=ClassT "IntBoxS" []]> lty)).
 
 Lemma Main_ty lty :
   cmd_has_ty lty ProgramBody (final_lty lty).
 Proof.
   rewrite /final_lty /ProgramBody.
   eapply SeqTy.
-  { eapply NewTy.
-    + by apply has_fields_BoxInt.
+  { eapply NewTy with (targs := []).
+    + by econstructor.
+    + by apply has_fields_IntBoxS.
     + by set_solver.
     + move => f fty arg.
       rewrite !lookup_insert_Some.
@@ -209,9 +266,9 @@ Proof.
     + econstructor.
       by rewrite lookup_insert.
     + by apply has_method_get.
-    + rewrite /BoxIntGet /=.
+    + rewrite /BoxGet /=.
       by set_solver.
-    + by move => x ty arg; rewrite /BoxIntGet /= lookup_empty.
+    + by move => x ty arg; rewrite /BoxGet /= lookup_empty.
   }
   eapply SeqTy.
   { eapply LetTy.
@@ -226,9 +283,9 @@ Proof.
       rewrite lookup_insert_ne //.
       by rewrite lookup_insert.
     + by apply has_method_set.
-    + rewrite /BoxIntGet /=.
+    + rewrite /BoxGet /=.
       by set_solver.
-    + move => x ty arg; rewrite /BoxIntGet /= lookup_insert_Some.
+    + move => x ty arg; rewrite /BoxGet /= lookup_insert_Some.
       case => [[<- <-]|[? ?]].
       * rewrite lookup_insert => [= <-].
         constructor; first done.
@@ -237,9 +294,9 @@ Proof.
       * rewrite lookup_insert_Some.
         case => [[? ?]| [? ?]]; by simplify_eq.
   }
-  rewrite /BoxIntSet /=.
+  rewrite /IntBoxSSet /=.
   eapply SubTy; last first.
-  - eapply GetTy; last by apply has_fields_BoxInt.
+  - eapply GetTy; last by apply has_fields_IntBoxS.
     constructor.
     do 3 (rewrite lookup_insert_ne //).
     by rewrite lookup_insert.
@@ -258,8 +315,8 @@ Proof.
       destruct (decide (v = "$box")) as [-> | ?].
       { rewrite lookup_insert.
         rewrite lookup_insert_ne // lookup_insert in h.
-        case : h => ->.
-        by exists ty.
+        case : h => <-.
+        by eexists.
       }
       rewrite lookup_insert_ne // in h.
       rewrite lookup_insert_ne // in h.
@@ -267,53 +324,292 @@ Proof.
       by rewrite lookup_insert_ne.
 Qed.
 
+
+Lemma helper_ext: ∀ A B σ0, extends_using A B σ0 → A = "IntBoxS" ∧ B = "Box" ∧ σ0 = σ.
+Proof.
+  move => A B σ0 h; inv h.
+  rewrite /Δ /= lookup_insert_Some in H.
+  destruct H as [[<- <-] | [? H]].
+  + by rewrite /Box in H0.
+  + rewrite lookup_insert_Some in H.
+    destruct H as [[<- <-] | [? H]]; last by rewrite lookup_empty in H.
+    rewrite /IntBoxS /= in H0; by simplify_eq.
+Qed.
+
+Lemma helper_in_Box : ∀ T σt, inherits_using "Box" T σt → T = "Box" ∧ σt = [GenT 0].
+Proof.
+  move => T σt h; inv h.
+  + rewrite /Δ /= lookup_insert in H.
+    by simplify_eq.
+  + apply helper_ext in H.
+    destruct H; discriminate.
+  + apply helper_ext in H.
+    destruct H; discriminate.
+Qed.
+
+Lemma helper_in_IntBoxS : ∀ T σt, inherits_using "IntBoxS" T σt →
+  (T = "IntBoxS" ∧ σt = []) ∨
+  (T = "Box" ∧ σt = σ).
+Proof.
+  move => T σt h; inv h.
+  + rewrite /Δ /= lookup_insert_ne // lookup_insert in H.
+    left.
+    by simplify_eq.
+  + apply helper_ext in H.
+    destruct H; right; by simplify_eq.
+  + apply helper_ext in H.
+    destruct H as [_ [-> ->]]; right.
+    apply helper_in_Box in H0 as [-> ->].
+    done.
+Qed.
+
+Lemma helper_in: ∀ A B σ0, inherits_using A B σ0 →
+     (A = "IntBoxS" ∧ B = "Box" ∧ σ0 = σ) ∨
+     (A = "IntBoxS" ∧ B = "IntBoxS" ∧ σ0 = []) ∨
+     (A = "Box" ∧ B = "Box" ∧ σ0 = [GenT 0]).
+Proof.
+  move => A B σ0 h.
+  inv h.
+  + rewrite /Δ /= lookup_insert_Some in H.
+    destruct H as [[<- ?]|[? H]]; first (right; right; by rewrite -H).
+    rewrite lookup_insert_Some in H.
+    destruct H as [[<- ?]|[? H]]; first (right; left; by rewrite -H).
+    by rewrite lookup_empty in H.
+  + apply helper_ext in H as [-> [-> ->]].
+    by left.
+  + apply helper_ext in H as [-> [-> ->]].
+    apply helper_in_Box in H0 as [-> ->].
+    by left.
+Qed.
+
 Lemma wf: wf_cdefs Δ.
 Proof.
   rewrite /Δ /=.
   split.
-  - apply map_Forall_singleton.
-    by rewrite /wf_cdef_fields /BoxInt /= => f fty super.
-  - apply map_Forall_singleton.
-    by rewrite /wf_cdef_methods /BoxInt /=.
-  - apply map_Forall_singleton.
-    rewrite /BoxInt /=.
-    apply map_Forall_lookup => m mdef.
+  - move => A B σ0 σ1 h0 h1.
+    apply helper_in in h0.
+    destruct h0 as [[-> [-> ->]] | [[-> [-> ->]] | [-> [-> ->]]]].
+    + apply helper_in_Box in h1; by destruct h1; discriminate.
+    + apply helper_in_IntBoxS in h1 as [[_ ->] | [h ?]]; last discriminate.
+      done.
+    + apply helper_in_Box in h1 as [_ ->].
+      done.
+  - apply map_Forall_lookup => c0 d0.
     rewrite lookup_insert_Some.
-    case => [[? ?] | [? h]]; simplify_eq.
-    + rewrite /BoxIntSet /wf_mdef_ty /=.
-      eexists; split; last by constructor.
+    case => [[? <-] | [?]] => //.
+    rewrite lookup_insert_Some.
+    case => [[? <-] | [?]] => //.
+    exists Box;repeat split => //.
+    + by apply wfσ.
+    + by apply σbounded.
+  - move => A B adef bdef m σ0 mA mB hA hB hin hmA hmB.
+    apply helper_in in hin.
+    destruct hin as [[-> [-> ->]] | [[-> [-> ->]] | [-> [-> ->]]]]; first last.
+    + simplify_eq.
+      rewrite /Δ /= lookup_insert in hA.
+      injection hA; intros; subst; clear hA.
+      rewrite /Box /= in hmA.
+      rewrite lookup_insert_Some in hmA.
+      destruct hmA as [[<- <-]|[? hmA]].
+      * rewrite /mdef_incl /BoxSet /subst_mdef /=.
+        split; first by set_solver.
+        split; last done.
+        move => k A B.
+        rewrite lookup_insert_Some.
+        case => [[<- <-]|[?]]; last by rewrite lookup_empty.
+        rewrite lookup_fmap lookup_insert /=.
+        by case => <-.
+      * rewrite lookup_insert_Some in hmA.
+        destruct hmA as [[<- <-]|[? hmA]]; last by rewrite lookup_empty in hmA.
+        rewrite /mdef_incl /BoxGet /subst_mdef /=.
+        split; first by set_solver.
+        split; last done.
+        move => k A B.
+        by rewrite lookup_empty.
+    + simplify_eq.
+      rewrite /Δ /= lookup_insert_ne // lookup_insert in hA.
+      injection hA; intros; subst; clear hA.
+      rewrite /IntBoxS /= in hmA.
+      rewrite lookup_insert_Some in hmA.
+      destruct hmA as [[<- <-]|[? hmA]]; last by rewrite lookup_empty in hmA.
+      rewrite /mdef_incl /IntBoxSSet /subst_mdef /=.
+      split; first by set_solver.
+      split; last done.
+      move => k A B.
+      rewrite lookup_insert_Some.
+      case => [[<- <-]|[?]]; last by rewrite lookup_empty.
+      rewrite lookup_fmap lookup_insert /=.
+      by case => <-.
+    + rewrite /Δ /= in hA, hB.
+      rewrite lookup_insert_ne // in hA.
+      rewrite !lookup_insert in hA, hB.
+      injection hA; injection hB; intros; subst; clear hA hB.
+      rewrite /IntBoxS /= in hmA.
+      rewrite /Box /= in hmB.
+      rewrite lookup_insert_Some in hmA.
+      destruct hmA as [[<- <-]|[? hmA]]; last by rewrite lookup_empty in hmA.
+      rewrite lookup_insert in hmB.
+      injection hmB; intros; subst; clear hmB.
+      rewrite /mdef_incl /IntBoxSSet /BoxSet /subst_mdef /σ /=.
+      split; first by set_solver.
+      split; last done.
+      move => k A B.
+      rewrite lookup_insert_Some.
+      case => [[<- <-]|[?]]; last by rewrite lookup_empty.
+      rewrite lookup_fmap_Some.
+      case => [ty [<-]].
+      rewrite lookup_insert.
+      by case => <-.
+  - rewrite map_Forall_lookup => c0 d0.
+    rewrite lookup_insert_Some.
+    case => [[? <-]|[?]].
+    { by rewrite /wf_cdef_fields /Box. }
+    rewrite lookup_insert_Some.
+    case => [[? <-]|[?]]; last by rewrite lookup_empty.
+    by rewrite /wf_cdef_fields /IntBoxS.
+  - rewrite map_Forall_lookup => c0 d0.
+    rewrite lookup_insert_Some.
+    case => [[? <-]|[?]].
+    { rewrite /wf_cdef_fields_bounded /Box /=.
+      rewrite map_Forall_singleton.
       econstructor.
-      * constructor.
-        by rewrite lookup_insert.
-      * constructor.
-        by rewrite lookup_insert_ne.
-      * by eauto.
-    + rewrite /wf_mdef_ty /=.
-      rewrite lookup_insert_Some in h.
-      destruct h as [[<- <-]|[hne hin]].
-      * rewrite /BoxIntGet /=.
-        eexists; split.
-        { econstructor.
+      by auto with arith.
+    }
+    rewrite lookup_insert_Some.
+    case => [[? <-]|[?]]; last by rewrite lookup_empty.
+    rewrite /wf_cdef_fields_bounded /IntBoxS /=.
+    by apply map_Forall_empty.
+  - rewrite map_Forall_lookup => c0 d0.
+    rewrite lookup_insert_Some.
+    case => [[? <-]|[?]].
+    { rewrite /wf_cdef_fields_wf /Box /=.
+      rewrite map_Forall_singleton.
+      by econstructor.
+    }
+    rewrite lookup_insert_Some.
+    case => [[? <-]|[?]]; last by rewrite lookup_empty.
+    rewrite /wf_cdef_fields_bounded /IntBoxS /=.
+    by apply map_Forall_empty.
+  - rewrite map_Forall_lookup => c0 d0.
+    rewrite lookup_insert_Some.
+    case => [[? <-]|[?]].
+    { rewrite /cdef_methods_bounded /Box /=.
+      rewrite map_Forall_lookup => x mx.
+      rewrite lookup_insert_Some.
+      case => [[? <-]|[?]].
+      + split; last by constructor.
+        rewrite /BoxSet /=.
+        rewrite map_Forall_singleton.
+        constructor.
+        by auto with arith.
+      + rewrite lookup_insert_Some.
+        case => [[? <-]|[?]]; last by rewrite lookup_empty.
+        split.
+        * rewrite /BoxGet /=.
+          by apply map_Forall_empty.
+        * rewrite /BoxGet /=.
           constructor.
+          by auto with arith.
+    }
+    rewrite lookup_insert_Some.
+    case => [[? <-]|[?]]; last by rewrite lookup_empty.
+    rewrite /cdef_methods_bounded /IntBoxS /=.
+    rewrite map_Forall_singleton.
+    split; last done.
+    rewrite /IntBoxSSet /=.
+    rewrite map_Forall_singleton.
+    by constructor.
+  - rewrite map_Forall_lookup => c0 d0.
+    rewrite lookup_insert_Some.
+    case => [[? <-]|[?]].
+    { rewrite /wf_cdef_methods_wf /Box /=.
+      rewrite map_Forall_lookup => x mx.
+      rewrite lookup_insert_Some.
+      case => [[? <-]|[?]].
+      + split; last by constructor.
+        rewrite /BoxSet /=.
+        rewrite map_Forall_singleton.
+        by constructor.
+      + rewrite lookup_insert_Some.
+        case => [[? <-]|[?]]; last by rewrite lookup_empty.
+        split.
+        * rewrite /BoxGet /=.
+          by apply map_Forall_empty.
+        * rewrite /BoxGet /=.
+          by constructor.
+    }
+    rewrite lookup_insert_Some.
+    case => [[? <-]|[?]]; last by rewrite lookup_empty.
+    rewrite /wf_cdef_methods_wf /IntBoxS /=.
+    rewrite map_Forall_singleton.
+    split.
+    + rewrite /IntBoxSSet /=.
+      rewrite map_Forall_singleton.
+      by constructor.
+    + rewrite /IntBoxSSet /=.
+      by constructor.
+  - rewrite map_Forall_lookup => c0 d0.
+    rewrite lookup_insert_Some.
+    case => [[<- <-]|[?]].
+    + rewrite /cdef_wf_mdef_ty /Box /=.
+      rewrite map_Forall_lookup => x mx.
+      rewrite lookup_insert_Some.
+      case => [[? <-]|[?]].
+      * rewrite /wf_mdef_ty /BoxSet /=.
+        eexists; split; last by constructor.
+        eapply SetTy.
+        { constructor.
           by rewrite lookup_insert.
-          by eauto.
+        }
+        { by eapply HasField. }
+        { constructor.
+          by rewrite lookup_insert_ne.
+        }
+      * rewrite lookup_insert_Some.
+        case => [[? <-]|[?]]; last by rewrite lookup_empty.
+        rewrite /wf_mdef_ty /BoxGet /=.
+        eexists; split.
+        { eapply GetTy.
+          { constructor.
+            by rewrite lookup_insert.
+          }
+          by eapply HasField.
         }
         constructor.
         by rewrite lookup_insert.
-      * by rewrite lookup_empty in hin.
+    + rewrite lookup_insert_Some.
+      case => [[<- <-]|[?]]; last by rewrite lookup_empty.
+      rewrite /cdef_wf_mdef_ty /IntBoxS /=.
+      rewrite map_Forall_singleton.
+      eexists; split; last by constructor.
+      rewrite /IntBoxSSet /=.
+      eapply SetTy.
+      * constructor.
+        by rewrite lookup_insert.
+      * eapply InheritsField => //.
+        by eapply HasField.
+      * constructor => //.
+        { constructor.
+          by rewrite lookup_insert_ne.
+        }
+        by constructor.
 Qed.
 
+(* Director level theorem: every execution that should produce an int
+ * actually produces an int.
+ *)
 Theorem int_adequacy cmd st lty n:
   cmd_eval (∅, ∅) cmd st n →
   cmd_has_ty ∅ cmd lty →
   ∀ v, lty !! v = Some IntT →
   ∃ z, st.1 !! v = Some (IntV z).
 Proof.
+  assert (wfemp : map_Forall (λ _ : string, wf_ty) ∅) by apply map_Forall_empty.
   move => he ht v hin.
   apply (@step_updN_soundness sem_heapΣ n).
   iMod sem_heap_init as (Hheap) "Hemp".
   iModIntro.
-  iDestruct ((cmd_adequacy _ _ _ wf ht _ _ _ he) with "Hemp") as "H" => /=.
+  iDestruct ((cmd_adequacy interp_env_empty _ _ _ wf wfemp ht _ _ _ he) with "Hemp") as "H" => /=.
   iRevert "H".
   iApply updN_mono.
   iIntros "[Hh Hl]".
