theories/interp.v
@@ -4,7 +4,7 @@
  * This source code is licensed under the MIT license found in the
  * LICENSE file in the root directory of this source tree.
  *)
-From stdpp Require Import base strings gmap stringmap fin_maps.
+From stdpp Require Import base strings gmap stringmap fin_maps natmap.
 From iris.base_logic Require Import upred derived.
 From iris.base_logic.lib Require Import iprop own.
 From iris.algebra Require Import ofe cmra gmap_view.
@@ -15,11 +15,15 @@ From shack Require Import lang heap modality.
 (* the interpretation of types is simply given by
      the carrier set of the sem_typeO ofe *)
 Record interp Σ := Interp {
-    interp_car :> value → iPropO Σ;
+    interp_car :> sem_typeO Σ;
     interp_persistent v : Persistent (interp_car v)
   }.
 
-Lemma interp_car_unfold : ∀ Σ c p, @interp_car Σ (Interp _ c p) = c.
+Definition interp_fun Σ (i: interp Σ) : value → iPropO Σ := interp_car Σ i.
+
+Coercion interp_fun : interp >-> Funclass.
+
+Lemma interp_car_simpl : ∀ Σ c p, @interp_car Σ (Interp _ c p) = c.
 Proof.
   by intros.
 Qed.
@@ -53,6 +57,9 @@ Section interp_cofe.
   Global Instance interp_car_ne n : Proper (dist n ==> (=) ==> dist n) interp_car.
   Proof. by intros A A' ? w ? <-. Qed.
 
+  Global Instance interp_car_ne2 : NonExpansive interp_car.
+  Proof. by move => n i j h. Qed.
+
   Global Instance interp_car_proper : Proper ((≡) ==> (=) ==> (≡)) interp_car.
   Proof. by intros A A' ? w ? <-. Qed.
 End interp_cofe.
@@ -73,10 +80,12 @@ Section proofs.
   Local Notation "lty <:< rty" := (@lty_sub _ lty rty) (at level 70, no associativity).
 
   (* now, let's interpret some types ! *)
-  Definition interp_null_car (v: value) : iProp Σ := ⌜v = NullV⌝%I.
-  Definition interp_null_persistent v : Persistent (interp_null_car v).
-  Proof. by apply _. Qed.
 
+  (* Most interpretation functions are parametrized by σi: tvar -> interp.
+   * This environment is here to interpret generic types.
+   * We could only consider closed types and eagerly apply all top level
+   * substitution, but this way makes things a bit more compositional.
+   *)
   Definition interp_null : interp Σ :=
     Interp (λ(v: value), ⌜v = NullV⌝%I).
 
@@ -95,105 +104,192 @@ Section proofs.
   Definition interp_nothing : interp Σ :=
     Interp (λ (_: value), False%I).
 
-  Notation ty_interpO := (lang_ty -d> sem_typeO Σ).
+   Notation ty_interpO := (lang_ty -d> listO (interpO Σ) -n> interpO Σ).
 
-  Definition interp_fields (rec: ty_interpO) (ftys: stringmap lang_ty) :
-    gmapO string (laterO (sem_typeO Σ)) :=
-    let f := λ (typ: lang_ty), Next (rec typ) in
-    @fmap _ _ _ (later (sem_typeO Σ)) f ftys
-  .
+   Lemma ty_interpO_ne : ∀ (rec: ty_interpO) ty, NonExpansive (rec ty).
+   Proof.
+     move => rec ty.
+     apply _.
+   Qed.
 
-  Lemma interp_fields_contractive ftys:
-    Contractive (λ f, interp_fields f ftys).
-  Proof.
-    move => n i1 i2 hdist.
-    rewrite /interp_fields.
-    apply gmap_fmap_ne_ext => k ty hin.
-    f_contractive.
-    by destruct n.
-  Qed.
+  Definition interp_fields
+    (σi: list (interp Σ))
+    (C: tag)
+    σC
+    (fields: stringmap lang_ty)
+    (ifields: gmapO string (laterO (sem_typeO Σ)))
+    (rec: ty_interpO) : iProp Σ :=
+    (⌜dom stringset fields = dom _ ifields⌝ ∗
+    ∀ f ty, ⌜has_field f C ty⌝ -∗ ifields !! f ≡ Some (Next (interp_car (rec (subst_ty σC ty) σi))))%I.
 
-  (* interpret a class type given the tag and the
-     interpretation of their fields *)
-  Definition interp_class (cname : tag) (rec : ty_interpO) : interp Σ :=
+  Definition interp_class C σC (σi: list (interp Σ)) (rec : ty_interpO) : interp Σ :=
     Interp (
       λ (w : value),
-      (∃ ℓ t (fields:stringmap lang_ty),
-      ⌜w = LocV ℓ ∧ inherits t cname ∧ has_fields t fields⌝ ∗
-      (ℓ ↦ (t , interp_fields rec fields)))%I
+      (∃ ℓ t σ σt (fields: stringmap lang_ty) (ifields: gmapO string (laterO (sem_typeO Σ))),
+      ⌜w = LocV ℓ ∧ inherits_using t C σ ∧ wf_ty (ClassT t σt) ∧ σC = subst_ty σt <$> σ ∧ has_fields t fields⌝ ∗
+      interp_fields σi t σt fields ifields rec ∗
+      (ℓ ↦ (t, ifields)))%I
     ).
 
-  Definition interp_nonnull (rec : ty_interpO) : interp Σ :=
+  Definition interp_ex σi (cname: tag) (rec: ty_interpO): interp Σ :=
+    Interp (λ (w: value), (∃ σc, interp_class cname σc σi rec w)%I).
+
+  Definition interp_nonnull σi (rec : ty_interpO) : interp Σ :=
     Interp (
       λ (v : value),
       ((interp_int v) ∨
       (interp_bool v) ∨
-      (∃ t, interp_class t rec v))%I
+      (∃ t, interp_ex σi t rec v))%I
     ).
 
-  Definition interp_mixed (rec: ty_interpO) : interp Σ :=
-    Interp (λ (v: value), (interp_nonnull rec v ∨ interp_null v)%I).
+  Definition interp_mixed σi (rec: ty_interpO) : interp Σ :=
+    Interp (λ (v: value), (interp_nonnull σi rec v ∨ interp_null v)%I).
+
+  Definition interp_generic (σi: list (interpO Σ)) (tv: nat) : interp Σ :=
+    default interp_nothing (σi !! tv).
 
   (* we use a blend of Coq/Iris recursion, the
      Coq recursion lets us handle simple structural
      cases, and we use Iris' recursion to deal with
-     the more complicated case of class types *)
-  Definition interp_type_pre (rec : ty_interpO) : ty_interpO :=
-    λ (typ : lang_ty),
-    (fix go (typ : lang_ty) : interp Σ :=
-    match typ with
-    | IntT => interp_int
-    | BoolT => interp_bool
-    | NothingT => interp_nothing
-    | MixedT => interp_mixed rec
-    | ClassT t => interp_class t rec
-    | NullT => interp_null
-    | NonNullT => interp_nonnull rec
-    | UnionT A B => interp_union (go A) (go B)
-    | InterT A B => interp_inter (go A) (go B)
-    end) typ.
+     the more complicated case of class types.
+  *)
+  Section interp_type_pre_rec.
+    Variable (σi: listO (interpO Σ)).
+    Variable (rec: ty_interpO).
 
-  Lemma interp_class_contractive cname:
-    Contractive (interp_class cname).
+    Fixpoint go (typ: lang_ty) : interp Σ :=
+      match typ with
+      | IntT => interp_int
+      | BoolT => interp_bool
+      | NothingT => interp_nothing
+      | MixedT => interp_mixed σi rec
+      | ClassT A σA => interp_class A σA σi rec
+      | NullT => interp_null
+      | NonNullT => interp_nonnull σi rec
+      | UnionT A B => interp_union (go A) (go B)
+      | InterT A B => interp_inter (go A) (go B)
+      | GenT n => interp_generic σi n
+      | ExT cname => interp_ex σi cname rec
+      end.
+  End interp_type_pre_rec.
+
+  Local Instance interp_class_ne cname σc (rec: ty_interpO) :
+    NonExpansive (λ σi, interp_class cname σc σi rec).
   Proof.
-    rewrite /interp_class => n i1 i2 hdist v.
-    rewrite !interp_car_unfold.
-    f_equiv ; intro l.
-    f_equiv; intro t.
-    f_equiv; intro fields.
-    f_equiv.
-    set (f := λ i, interp_fields i fields).
-    assert (hf : Contractive f) by apply interp_fields_contractive.
-    by apply (mapsto_contractive _ _ f).
+    move => n x y h.
+    rewrite /interp_class => v.
+    rewrite /interp_fun !interp_car_simpl.
+    do 13 f_equiv.
+    rewrite /interp_fields.
+    do 10 f_equiv.
+    by apply ty_interpO_ne.
   Qed.
 
-  Lemma interp_nonnull_contractive: Contractive interp_nonnull.
+  Local Instance interp_ex_ne cname (rec: ty_interpO) :
+    NonExpansive (λ σi, interp_ex σi cname rec).
+  Proof.
+    move => n x y h.
+    rewrite /interp_ex => v.
+    rewrite /interp_fun !interp_car_simpl.
+    do 3 f_equiv.
+    by apply interp_class_ne.
+  Qed.
+
+  Local Instance interp_nonnull_ne (rec: ty_interpO) :
+    NonExpansive (λ σi, interp_nonnull σi rec).
+  Proof.
+    move => n x y h.
+    rewrite /interp_nonnull => v.
+    rewrite /interp_fun !interp_car_simpl.
+    do 5 f_equiv.
+    by apply interp_ex_ne.
+  Qed.
+
+  Local Instance go_ne (rec: ty_interpO) (ty: lang_ty) :
+    NonExpansive (λ σi, go σi rec ty).
+  Proof.
+    induction ty as [ | | | | A σ hi | | | A B hA hB | A B hA hB | i | cname ] => //= n x y h.
+    - rewrite /interp_mixed => v.
+      rewrite /interp_fun !interp_car_simpl.
+      do 5 f_equiv.
+      by apply interp_ex_ne.
+    - by apply interp_class_ne.
+    - by apply interp_nonnull_ne.
+    - rewrite /interp_union => v.
+      rewrite /interp_fun !interp_car_simpl.
+      f_equiv.
+      + revert v; by apply hA.
+      + revert v; by apply hB.
+    - rewrite /interp_inter => v.
+      rewrite /interp_fun !interp_car_simpl.
+      f_equiv.
+      + revert v; by apply hA.
+      + revert v; by apply hB.
+    - rewrite /interp_generic => v.
+      assert (hl: length x = length y) by now apply Forall2_length in h.
+      elim : x y i h hl => [ | hd tl hi]; case => [ | hd' tl'] i h /= hl => //.
+      apply Forall2_cons in h as [hhd htl].
+      case: i hi => [ | i ] hi //=.
+      apply:  hi; first done.
+      by lia.
+    - by apply interp_ex_ne.
+  Qed.
+
+  (* TODO: find a better name for go *)
+  Definition interp_type_pre (rec : ty_interpO) : ty_interpO :=
+    λ (typ : lang_ty), λne (σi: listO (interpO Σ)), go σi rec typ.
+
+  Global Instance interp_type_pre_persistent (rec: ty_interpO) :
+    ∀ t σi v, Persistent (interp_type_pre rec t σi v).
+  Proof. by move => ???; apply _. Qed.
+
+  Global Instance interp_class_contractive cname σc σi:
+    Contractive (interp_class cname σc σi). 
+  Proof.
+    rewrite /interp_class => n i1 i2 hdist v.
+    rewrite /interp_fun !interp_car_simpl.
+    do 6 (f_equiv; intros ?).
+    f_equiv.
+    rewrite /interp_fields.
+    do 9 f_equiv.
+    f_contractive.
+    apply interp_car_ne2.
+    by f_equiv.
+  Qed.
+
+  Global Instance interp_ex_contractive σi cname: Contractive (interp_ex σi cname).
+  Proof.
+    rewrite /interp_ex => n i1 i2 hdist v.
+    rewrite /interp_fun !interp_car_simpl.
+    do 2 f_equiv.
+    by apply interp_class_contractive.
+  Qed.
+
+  Global Instance interp_nonnull_contractive σi: Contractive (interp_nonnull σi).
   Proof.
     rewrite /interp_nonnull => n i1 i2 hdist v.
-    rewrite !interp_car_unfold.
+    rewrite /interp_fun !interp_car_simpl.
     do 4 f_equiv.
-    revert v.
-    by apply interp_class_contractive.
+    by apply interp_ex_contractive.
   Qed.
 
   (* we cannot use solve_contractive out of the box because of
    * the 'fix' combinator above
    *)
-  Local Instance interp_type_pre_contractive:
-  Contractive (interp_type_pre).
+  Local Instance interp_type_pre_contractive : Contractive interp_type_pre.
   Proof.
-    move => n i1 i2 hdist.
-    move => ty.
-    elim : ty; intros; rewrite /interp_type_pre //=;
-    [ (* mixed *)| (*class*) | (*nonnull*) 
-    | solve_proper_core ltac:(fun _ => first [done | f_contractive | f_equiv])
-    | solve_proper_core ltac:(fun _ => first [done | f_contractive | f_equiv])
-    ].
-     - move => v; rewrite /interp_mixed !interp_car_unfold.
-       f_equiv; revert v.
-       by apply interp_nonnull_contractive.
-     - by apply interp_class_contractive.
-     - by apply interp_nonnull_contractive.
+    rewrite /interp_type_pre => n rec1 rec2 hdist ty σi /=.
+    induction ty
+      as [ | | | | cname σ hi | | | A B hA hB | A B hA hB | i | cname ] => //=.
+    - rewrite /interp_mixed => v.
+      rewrite /interp_fun !interp_car_simpl.
+      f_equiv.
+      revert v; by apply interp_nonnull_contractive.
+    - by apply interp_class_contractive.
+    - by apply interp_nonnull_contractive.
+    - solve_proper_core ltac:(fun _ => first [done | f_contractive | f_equiv]).
+    - solve_proper_core ltac:(fun _ => first [done | f_contractive | f_equiv]).
+    - by apply interp_ex_contractive.
   Qed.
 
   (* the interpretation of types can now be
@@ -201,80 +297,172 @@ Section proofs.
      can be (mutually) recursive) *)
   Definition interp_type := fixpoint interp_type_pre.
 
-  Lemma interp_type_unfold (ty : lang_ty) (v : value) :
-    interp_type ty v ⊣⊢ interp_type_pre interp_type ty v.
+  Record interp_env := InterpEnv {
+    interp_env_car :> list (interpO Σ);
+    interp_env_as_mixed:
+      Forall (λ (e: interp Σ), ∀ v, e v -∗ interp_mixed interp_env_car interp_type v) interp_env_car
+  }.
+
+  Definition interp_env_empty : interp_env := InterpEnv [] (Forall_nil_2 _).
+
+  (* Helper lemmas to control unfolding of some definitions *)
+  Lemma interp_type_unfold (σi: list (interpO Σ)) (ty : lang_ty) (v : value) :
+    interp_type ty σi v ⊣⊢ interp_type_pre interp_type ty σi v.
   Proof.
     rewrite {1}/interp_type.
-    apply (fixpoint_unfold interp_type_pre ty v).
+    apply (fixpoint_unfold interp_type_pre ty σi v).
+  Qed.
+
+  Lemma interp_ex_unfold σi t v:
+    interp_type (ExT t) σi v ⊣⊢ interp_ex σi t interp_type v.
+  Proof. by rewrite interp_type_unfold /= /interp_ex /=. Qed.
+
+  Lemma interp_nonnull_unfold σi v:
+    interp_type NonNullT σi v ⊣⊢
+      (interp_int v) ∨ (interp_bool v) ∨ (∃ t, interp_ex σi t interp_type v)%I.
+  Proof. by rewrite interp_type_unfold /= /interp_nonnull /=. Qed.
+
+  Lemma interp_mixed_unfold σi v:
+    interp_type MixedT σi v ⊣⊢ interp_nonnull σi interp_type v ∨ interp_null v.
+  Proof. by rewrite interp_type_unfold /interp_mixed /=. Qed.
+
+  Lemma interp_class_unfold σi A σA v:
+    interp_type (ClassT A σA) σi v ⊣⊢
+    interp_class A σA σi interp_type v.
+  Proof. by rewrite interp_type_unfold. Qed.
+
+  Lemma interp_union_unfold σi A B v:
+    interp_type (UnionT A B) σi v ⊣⊢
+    interp_union (interp_type A σi) (interp_type B σi) v.
+  Proof.
+    rewrite interp_type_unfold /=.
+    iSplit; iIntros "[H | H]".
+    - iLeft; by rewrite interp_type_unfold.
+    - iRight; by rewrite interp_type_unfold.
+    - iLeft; by rewrite interp_type_unfold.
+    - iRight; by rewrite interp_type_unfold.
+  Qed.
+
+  Lemma interp_inter_unfold σi A B v:
+    interp_type (InterT A B) σi v ⊣⊢
+    interp_inter (interp_type A σi) (interp_type B σi) v.
+  Proof.
+    rewrite interp_type_unfold /=.
+    iSplit; iIntros "[HL HR]".
+    - rewrite !interp_type_unfold; by iSplit.
+    - rewrite !interp_type_unfold; by iSplit.
   Qed.
 
   (* #hyp *)
-  Global Instance interp_type_persistent : ∀ t v, Persistent (interp_type t v).
+  Global Instance interp_type_persistent :
+    ∀ t σi v, Persistent (interp_type t σi v).
   Proof.
-    elim => [ | | | | cname | | |s hs t ht | s hs t ht] v;
-        rewrite interp_type_unfold //=; try by apply _.
+    move => t σi v.
+    rewrite interp_type_unfold.
+    by apply _.
   Qed.
 
-  Lemma dom_interp_fields fields:
-    dom stringset (interp_fields interp_type fields) ≡ dom _ fields.
-  Proof. by rewrite /interp_fields dom_fmap. Qed.
-
-  Lemma inherits_is_inclusion:
-    ∀ A B, inherits A B →
-    ∀ v, interp_class A interp_type v -∗ interp_class B interp_type v.
+  (* if class A<..> extends B<σB>, then for any valid substitution σA,
+   * [| A<σA> |] ⊆ [| B<σA o σB> |]
+   *)
+  Lemma extends_using_is_inclusion:
+    map_Forall (λ _cname, wf_cdef_fields) Δ →
+    map_Forall (λ _cname, wf_cdef_fields_bounded) Δ →
+    map_Forall (λ _cname, wf_cdef_parent Δ) Δ →
+    ∀ A B σB, extends_using A B σB →
+    ∀ σi v σA, interp_type (ClassT A σA) σi v -∗
+    interp_type (ClassT B (subst_ty σA <$> σB)) σi v.
   Proof.
-    move => A B hAB v.
-    rewrite /interp_class.
+    move => hwf /map_Forall_lookup hwfb /map_Forall_lookup hwp A B σB hext σi v σA.
+    rewrite !interp_type_unfold /=.
     iIntros "h".
-    iDestruct "h" as (ℓ t fields) "[%h hsem]".
-    destruct h as [-> [hext2 hfields ]].
-    iExists ℓ, t, fields.
+    iDestruct "h" as (ℓ t σ σt fields ifields) "[%h [hsem hl]]".
+    destruct h as [-> [hin [hσwf [hσ hfields]]]].
+    rewrite /interp_fields.
+    iDestruct "hsem" as "[%hdom hsem]".
+    iExists ℓ, t, (subst_ty σ <$> σB), σt, fields, ifields. 
     iSplit.
-    { iPureIntro; split; first by done.
+    { iPureIntro; split; first done.
+      split.
+      { by eapply inherits_using_trans; last by econstructor. }
+      split; first done.
       split; last done.
-      by eapply rtc_transitive.
+      rewrite hσ map_subst_ty_subst //.
+      apply inherits_using_wf in hin => //.
+      destruct hin as (? & ? &? &? & ? & hL & _).
+      apply extends_using_wf in hext => //.
+      destruct hext as (? & ? & ? & ? & hF & ? & _).
+      clear hdom; simplify_eq.
+      by rewrite hL.
     }
-    by iFrame.
+    iSplit; last done.
+    iSplit; first by iPureIntro.
+    iIntros (f ty) "%hf".
+    by iApply "hsem".
   Qed.
 
-  (* A <: B → ΦA ⊂ ΦB *)
+  (* Main meat for A <: B → [|A|] ⊆ [|B|] *)
   Theorem subtype_is_inclusion_aux:
+    map_Forall (λ _cname, wf_cdef_fields) Δ →
+    map_Forall (λ _cname, wf_cdef_fields_bounded) Δ →
+    map_Forall (λ _cname, wf_cdef_parent Δ) Δ →
     ∀ (A B: lang_ty), A <: B →
-    ∀ v,
-    interp_type_pre interp_type A v -∗
-    interp_type_pre interp_type B v.
+    ∀ (env: interp_env) v,
+    interp_type_pre interp_type A env v -∗
+    interp_type_pre interp_type B env v.
   Proof.
-    induction 1 as [A | A B hext | | | | A | A B| A B | A B C h0 hi0 h1 hi1
-        | A B | A B | A B C h0 hi0 h1 hi1 | A | A B C h0 hi0 h1 hi1 ];
-    move => v /=.
+    move => ? ? ?.
+    induction 1 as [A | A h | A σA B σB adef hΔ hlen hext | | | | A | A B h
+      | A B h | A B C h0 hi0 h1 hi1 | A B | A B | A B C h0 hi0 h1 hi1
+      | A | A B C h0 hi0 h1 hi1 ];
+    move => env v.
     - rewrite /interp_mixed.
-      elim: A v => //=.
+      elim: A v => //.
       + move => v; iIntros "h"; by repeat iLeft.
       + move => v; iIntros "h"; by iLeft; iRight; iLeft.
       + move => v; by rewrite /interp_nothing; iIntros "h".
-      + move => cname v.
+      + move => cname targs _ v.
         iIntros "h".
         iLeft; iRight; iRight.
-        iExists cname; by iApply inherits_is_inclusion. 
+        by iExists cname, targs.
       + move => v; iIntros "h"; by iRight.
       + move => v; by iIntros "h"; iLeft.
-      + move => s hs t ht v.
+      + move => s t hs ht v.
         rewrite /interp_union.
         iIntros "h".
         iDestruct "h" as "[ h | h ]"; first by iApply hs.
         by iApply ht.
-      + move => s hs t ht v.
+      + move => s t hs ht v.
         rewrite /interp_inter.
         iIntros "h".
         iDestruct "h" as "[? _]"; by iApply hs.
-    - by iApply inherits_is_inclusion.
+      + move => n v.
+        rewrite /interp_generic.
+        iIntros "hv".
+        destruct env as [env henv] => /=.
+        rewrite Forall_forall in henv.
+        destruct (decide (n < length env)) as [hlt | hge].
+        * iApply henv; last done.
+          apply lookup_lt_is_Some_2 in hlt as [ t ht ].
+          rewrite /interp_generic ht /=.
+          by apply elem_of_list_lookup_2 in ht.
+        * rewrite /interp_generic lookup_ge_None_2 /=; last by apply not_lt.
+          done.
+      + move => cname v;
+        rewrite /interp_ex.
+        iIntros "hv".
+        iDestruct "hv" as (targs) "hv".
+        iLeft; iRight; iRight.
+        by iExists _, _.
+    - rewrite /=.
+      by iIntros "H".
+    - by rewrite -!interp_type_unfold; iApply extends_using_is_inclusion.
     - by rewrite /= /interp_mixed.
     - iIntros "h"; by iLeft.
     - iIntros "h"; by iRight; iLeft.
     - iIntros "H".
       iRight; iRight.
-      iExists A.
-      by iApply inherits_is_inclusion.
+      by iExists A, _.
     - rewrite /interp_union.
       by iIntros "h"; iLeft.
     - rewrite /interp_union.
@@ -292,33 +480,94 @@ Section proofs.
       by iApply hi1.
     - done.
     - iIntros "h".
-      iApply hi1.
-  by iApply hi0.
+      iApply hi1 => //.
+      by iApply hi0.
   Qed.
 
+  (* A <: B → [|A|] ⊆ [|B|] *)
   Theorem subtype_is_inclusion:
+    map_Forall (λ _cname, wf_cdef_fields) Δ →
+    map_Forall (λ _cname, wf_cdef_fields_bounded) Δ →
+    map_Forall (λ _cname, wf_cdef_parent Δ) Δ →
     ∀ A B, A <: B →
-    ∀ v, interp_type A v -∗ interp_type B v.
+    ∀ (env: interp_env),
+    ∀ v, interp_type A env v -∗ interp_type B env v.
   Proof.
-    move => A B hAB v.
+    move => ??? A B hAB env v.
     rewrite !interp_type_unfold.
     by iApply subtype_is_inclusion_aux.
   Qed.
 
-  Definition interp_local_tys
-    (lty : local_tys) (le : local_env) : iProp Σ :=
-    (∀ v ty, ⌜lty !! v = Some ty⌝ -∗
-    ∃ val, ⌜le !! v = Some val⌝ ∗ interp_type ty val)%I.
-
-  Lemma interp_local_tys_is_inclusion lty rty le:
-    lty <:< rty →
-    interp_local_tys lty le -∗
-    interp_local_tys rty le.
+  (* Specialized version for existential types. Will help during the
+   * proof of adequacy for runtime checks.
+   *)
+  Theorem inherits_is_ex_inclusion:
+    map_Forall (λ _cname, wf_cdef_fields) Δ →
+    map_Forall (λ _cname, wf_cdef_fields_bounded) Δ →
+    map_Forall (λ _cname, wf_cdef_parent Δ) Δ →
+    ∀ A B, inherits A B →
+    ∀ (env: interp_env),
+    ∀ v, interp_type (ExT A) env v -∗ interp_type (ExT B) env v.
   Proof.
-    move => hsub; iIntros "Hle" (v ty) "%Hv".
+    move => ???.
+    induction 1 as [ x | x y z hxy hyz hi ] => // σi v.
+    rewrite interp_ex_unfold.
+    iIntros "H".
+    iApply hi; clear hyz hi.
+    iDestruct "H" as (σx) "H".
+    inv hxy.
+    iAssert (interp_type (ClassT y (subst_ty σx <$> σB)) σi v) with "[H]" as "Hext".
+    { iApply extends_using_is_inclusion => //.
+      - by econstructor.
+      - by rewrite interp_class_unfold.
+    }
+    rewrite interp_class_unfold interp_ex_unfold.
+    by iExists (subst_ty σx <$> σB).
+  Qed.
+
+  Definition interp_local_tys
+    σi (lty : local_tys) (le : local_env) : iProp Σ :=
+    (∀ v ty, ⌜lty !! v = Some ty⌝ -∗
+    ∃ val, ⌜le !! v = Some val⌝ ∗ interp_type ty σi val)%I.
+
+  Lemma interp_local_tys_is_inclusion (σi: interp_env)  lty rty le:
+    map_Forall (λ _cname, wf_cdef_fields) Δ →
+    map_Forall (λ _cname, wf_cdef_fields_bounded) Δ →
+    map_Forall (λ _cname, wf_cdef_parent Δ) Δ →
+    Forall (λ (i: interp Σ), ∀ v, Persistent (i v)) σi →
+    lty <:< rty →
+    interp_local_tys σi lty le -∗
+    interp_local_tys σi rty le.
+  Proof.
+    move => ??? hpers hsub; iIntros "Hle" (v ty) "%Hv".
     apply hsub in Hv as (B & hB & hsubB).
     iDestruct ("Hle" $! v B hB) as (val) "[%Hv' #H]".
     iExists val; iSplitR; first done.
     by iApply subtype_is_inclusion.
+  Qed.
+
+  (* Helper to lift the conclusions of interp_class into a super class *)
+  Lemma interp_fields_inclusion σi t σt fields ifields σ C rec:
+    map_Forall (λ _cname, wf_cdef_parent Δ) Δ →
+    map_Forall (λ _cname, wf_cdef_fields) Δ →
+    map_Forall (λ _cname, wf_cdef_fields_bounded) Δ →
+    inherits_using t C σ →
+    interp_fields σi t σt fields ifields rec -∗
+    interp_fields σi C (subst_ty σt <$> σ) fields ifields rec.
+  Proof.
+    move => ?? hb hin.
+    rewrite /interp_fields.
+    iIntros "[%hdom #H]".
+    iSplit; first done.
+    iIntros (f ty) "%hf".
+    assert (hfC: has_field f t (subst_ty σ ty)) by (by eapply has_field_inherits_using).
+    iSpecialize ("H" $! f (subst_ty σ ty) hfC).
+    rewrite subst_ty_subst //.
+    apply has_field_bounded in hf => //.
+    destruct hf as (def & hdef & hfty).
+    apply inherits_using_wf in hin => //.
+    destruct hin as (? & ? & ? & ? & _ & hL & _).
+    simplify_eq.
+    by rewrite hL.
   Qed.
 End proofs.
