theories/lang.v
@@ -35,17 +35,173 @@ Inductive value : Set :=
   | LocV (ℓ : loc).
 Local Instance value_inhabited : Inhabited value := populate NullV.
 
-Inductive lang_ty :=
-  | IntT
-  | BoolT
-  | NothingT
-  | MixedT
-  | ClassT (cname: tag)
-  | NullT
-  | NonNullT
-  | UnionT (s t: lang_ty)
-  | InterT (s t: lang_ty)
+Section nested_ind.
+  Local Unset Elimination Schemes.
+
+  Inductive lang_ty :=
+    | IntT
+    | BoolT
+    | NothingT
+    | MixedT
+    | ClassT (cname: tag) (targs: list lang_ty)
+    | NullT
+    | NonNullT
+    | UnionT (s t: lang_ty)
+    | InterT (s t: lang_ty)
+    | GenT (n: nat)
+    | ExT (cname: tag) (* Ext C == ∃Ti, ClassT C Ti *) 
+  .
+
+  Variable P : lang_ty -> Prop.
+  Hypothesis case_IntT : P IntT.
+  Hypothesis case_BoolT : P BoolT.
+  Hypothesis case_NothingT : P NothingT.
+  Hypothesis case_MixedT : P MixedT.
+  Hypothesis case_ClassT : ∀ cname targs, Forall P targs → P (ClassT cname targs).
+  Hypothesis case_NullT : P NullT.
+  Hypothesis case_NonNullT : P NonNullT.
+  Hypothesis case_UnionT :  ∀ s t, P s → P t → P (UnionT s t).
+  Hypothesis case_InterT :  ∀ s t, P s → P t → P (InterT s t).
+  Hypothesis case_GenT: ∀ n, P (GenT n).
+  Hypothesis case_ExT: ∀ cname, P (ExT cname).
+
+  Fixpoint lang_ty_ind (t : lang_ty) :=
+    match t with
+    | IntT => case_IntT
+    | BoolT => case_BoolT
+    | NothingT => case_NothingT
+    | MixedT => case_MixedT
+    | ClassT cname targs =>
+        let H := (fix fold (xs : list lang_ty) : Forall P xs :=
+          match xs with
+          | nil => List.Forall_nil _
+          | x :: xs => List.Forall_cons _ x xs (lang_ty_ind x) (fold xs)
+          end) targs in
+        case_ClassT cname targs H
+    | NullT => case_NullT
+    | NonNullT => case_NonNullT
+    | UnionT s t => case_UnionT s t (lang_ty_ind s) (lang_ty_ind t)
+    | InterT s t => case_InterT s t (lang_ty_ind s) (lang_ty_ind t)
+    | GenT n => case_GenT n
+    | ExT cname => case_ExT cname
+    end.
+End nested_ind.
+
+(* A type is bounded by n if any generic that might be
+ * present in it is < n
+ *)
+Inductive bounded (n: nat) : lang_ty → Prop :=
+  | ClassIsBounded cname targs :
+      Forall (bounded n) targs → bounded n (ClassT cname targs)
+  | UnionIsBounded s t :
+      bounded n s → bounded n t → bounded n (UnionT s t)
+  | InterIsBounded s t :
+      bounded n s → bounded n t → bounded n (InterT s t)
+  | GenIsBounded k:
+      k < n → bounded n (GenT k)
+  | IntIsBounded : bounded n IntT
+  | BoolIsBounded : bounded n BoolT
+  | NothingIsBounded : bounded n NothingT
+  | MixedIsBounded : bounded n MixedT
+  | NullIsBounded : bounded n NullT
+  | NonNullIsBounded : bounded n NonNullT
+  | ExIsBounded cname : bounded n (ExT cname)
 .
+
+Global Hint Constructors bounded : core.
+
+(* To be used with `bounded`: Generics must be always bound *)
+Fixpoint subst_ty (targs:list lang_ty) (ty: lang_ty):  lang_ty :=
+  match ty with
+  | ClassT cname cargs => ClassT cname (subst_ty targs <$> cargs)
+  | UnionT s t => UnionT (subst_ty targs s) (subst_ty targs t)
+  | InterT s t => InterT (subst_ty targs s) (subst_ty targs t)
+  | GenT n => default ty (targs !! n)
+  | ExT _ | IntT | BoolT | NothingT | MixedT | NullT | NonNullT => ty
+  end.
+
+Lemma subst_ty_subst ty l k:
+  bounded (length k) ty →
+  subst_ty l (subst_ty k ty) = subst_ty (subst_ty l <$> k) ty.
+Proof.
+  move => hbounded.
+  induction ty as [ | | | | cname targs hi | | | s t hs ht |
+      s t hs ht | n | cname ] => //=.
+  - f_equal.
+    rewrite -list_fmap_compose.
+    rewrite Forall_forall in hi.
+    apply map_ext_in => s /elem_of_list_In hin.
+    apply hi => //.
+    inv hbounded.
+    rewrite Forall_forall in H0.
+    by apply H0.
+  - inv hbounded.
+    f_equal; by eauto.
+  - inv hbounded.
+    f_equal; by eauto.
+  - rewrite list_lookup_fmap.
+    destruct (k !! n) as [ ty | ] eqn:hty => //=.
+    inv hbounded.
+    apply lookup_lt_is_Some_2 in H0.
+    rewrite hty in H0.
+    by elim H0.
+Qed.
+
+Lemma map_subst_ty_subst (j k l: list lang_ty):
+  Forall (bounded (length k)) l →
+  subst_ty j <$> (subst_ty k <$> l) =
+  subst_ty (subst_ty j <$> k) <$> l.
+Proof.
+  move => hwf.
+  induction l as [ | hd tl hi] => //=.
+  inv hwf.
+  rewrite subst_ty_subst => //.
+  f_equal.
+  by rewrite list_fmap_compose -/subst_ty list_fmap_id -/fmap hi.
+Qed.
+
+Lemma fmap_subst_ty_subst j k (l: stringmap lang_ty):
+  map_Forall (λ _, bounded (length k)) l →
+  subst_ty j <$> (subst_ty k <$> l) =
+  subst_ty (subst_ty j <$> k) <$> l.
+Proof.
+  move => hwf.
+  move: j k hwf.
+  induction l as [| s ty ftys Hs IH] using map_ind => j k hwf;
+    first by rewrite !fmap_empty.
+  rewrite map_Forall_insert // in hwf.
+  destruct hwf as [hhd htl].
+  by rewrite !fmap_insert subst_ty_subst // IH.
+Qed.
+
+Lemma bounded_subst n ty:
+  bounded n ty →
+  ∀ m targs, length targs = n →
+  Forall (bounded m) targs →
+  bounded m (subst_ty targs ty).
+Proof.
+  induction ty as [ | | | | cname targs hi | | | s t hs ht |
+      s t hs ht | k | cname ] => //= hb m σ hlen hσ.
+  - constructor.
+    rewrite Forall_forall => ty /elem_of_list_fmap hin.
+    destruct hin as [ty' [-> hin]].
+    rewrite Forall_forall in hi.
+    apply hi with (m := m) (targs := σ) in hin => //.
+    inv hb.
+    rewrite Forall_forall in H0.
+    by apply H0.
+  - inv hb.
+    constructor; by eauto.
+  - inv hb.
+    constructor; by eauto.
+  - inv hb.
+    rewrite Forall_forall in hσ.
+    apply hσ.
+    apply lookup_lt_is_Some_2 in H0.
+    destruct (σ !! k) as [ ty | ] eqn:hty; last by elim H0.
+    by apply elem_of_list_lookup_2 in hty.
+Qed.
+
 Definition var := string.
 Global Instance var_dec_eq (l l' : var) : Decision (l = l') := _.
 
@@ -70,7 +226,7 @@ Inductive cmd : Set :=
   | NewC (lhs: var) (class_name: tag) (args: stringmap expr)
   | GetC (lhs: var) (recv: expr) (name: string)
   | SetC (recv: expr) (fld: string) (rhs: expr)
-      (* tag test "if ($v is C) { ... }" *)
+      (* tag test "if ($v is C<_>) { ... }" *)
   | CondTagC (v : var) (t : tag) (body : cmd)
 .
 
@@ -82,62 +238,541 @@ Record methodDef := {
   methodret: expr;
 }.
 
+Definition subst_mdef targs mdef : methodDef := {|
+    methodname := mdef.(methodname);
+    methodargs := subst_ty targs <$> mdef.(methodargs);
+    methodrettype := subst_ty targs mdef.(methodrettype);
+    methodbody := mdef.(methodbody);
+    methodret := mdef.(methodret);
+  |}.
+
+Lemma subst_mdef_body mdef σ: methodbody (subst_mdef σ mdef) = methodbody mdef.
+Proof. by []. Qed.
+
+Lemma subst_mdef_ret mdef σ: methodret (subst_mdef σ mdef) = methodret mdef.
+Proof. by []. Qed.
+
+Definition mdef_bounded n mdef : Prop :=
+  map_Forall (λ _argname, bounded n) mdef.(methodargs) ∧ bounded n mdef.(methodrettype).
+
+Lemma subst_mdef_mdef k l mdef :
+  mdef_bounded (length l) mdef →
+  subst_mdef k (subst_mdef l mdef) = subst_mdef (subst_ty k <$> l) mdef.
+Proof.
+  rewrite /mdef_bounded map_Forall_lookup.
+  case => hargs hret.
+  rewrite /subst_mdef; destruct mdef as [? args ret ? ?]; f_equiv => //=.
+  - by rewrite fmap_subst_ty_subst.
+  - by rewrite subst_ty_subst.
+Qed.
+
+Lemma bounded_subst_mdef n mdef:
+  mdef_bounded n mdef →
+  ∀ m targs, length targs = n →
+  Forall (bounded m) targs →
+  mdef_bounded m (subst_mdef targs mdef).
+Proof.
+  move => [/map_Forall_lookup hargs hret] m σ hl hf.
+  rewrite /mdef_bounded /subst_mdef /=; split; last by apply bounded_subst with n.
+  rewrite map_Forall_lookup => k ty hty.
+  apply lookup_fmap_Some in hty as [ty' [ <- hm]].
+  apply bounded_subst with n => //.
+  by eapply hargs.
+Qed.
+
 Record classDef := {
   classname: tag;
-  superclass: option tag;
+  generics: nat; (* number of generics, no constraint for now *)
+  superclass: option (tag * list lang_ty);
   classfields : stringmap lang_ty;
   classmethods : stringmap methodDef;
 }.
+
+(* "Identity" substitution for n generics *)
+Definition gen_targs n : list lang_ty := map GenT (seq 0 n).
+
+Lemma lookup_gen_targs_lt :
+  ∀ n pos, pos < n → gen_targs n !! pos = Some (GenT pos).
+Proof.
+  move => n pos h.
+  by rewrite /gen_targs list_lookup_fmap lookup_seq_lt.
+Qed.
+
+Lemma length_gen_targs n : length (gen_targs n) = n.
+Proof. by rewrite /gen_targs map_length seq_length. Qed.
+
+Lemma subst_ty_id n ty:
+  bounded n ty →
+  subst_ty (gen_targs n) ty = ty.
+Proof.
+  move => h.
+  induction ty as [ | | | | cname targs hi | | | s t hs ht |
+      s t hs ht | k | cname ] => //=.
+  - f_equal.
+    rewrite Forall_forall in hi.
+    pattern targs at 2.
+    replace targs with (map id targs) by apply map_id.
+    apply map_ext_in => /= s /elem_of_list_In hin.
+    apply hi => //.
+    inv h.
+    rewrite Forall_forall in H0.
+    by apply H0.
+  - inv h; f_equal; by eauto.
+  - inv h; f_equal; by eauto.
+  - inv h.
+    by rewrite lookup_gen_targs_lt.
+Qed.
+
+Lemma subst_tys_id n σ:
+  Forall (bounded n) σ →
+  subst_ty (gen_targs n) <$> σ = σ.
+Proof.
+  revert n.
+  induction σ as [ | hd tl hi] => σ //= hf.
+  f_equal.
+  - apply subst_ty_id.
+    apply Forall_inv in hf.
+    by apply hf.
+  - apply hi.
+    by apply Forall_inv_tail in hf.
+Qed.
+
+Lemma fmap_subst_tys_id n (m: stringmap lang_ty):
+  map_Forall (λ _, bounded n) m →
+  subst_ty (gen_targs n) <$> m = m.
+Proof.
+  revert n.
+  induction m as [| s ty ftys Hs IH] using map_ind => n hm; first by rewrite fmap_empty.
+  rewrite fmap_insert; f_equal.
+  - apply subst_ty_id.
+    apply hm with s.
+    by rewrite lookup_insert.
+  - apply IH.
+    rewrite map_Forall_lookup => k tk hk.
+    apply hm with k.
+    rewrite lookup_insert_ne // => heq; subst.
+    by rewrite Hs in hk.
+Qed.
+
+Lemma subst_ty_gen_targs n targs :
+  length targs = n →
+  subst_ty targs <$> (gen_targs n) = targs.
+Proof.
+  move => hlen.
+  apply nth_ext with NothingT NothingT.
+  - by rewrite map_length length_gen_targs.
+  - rewrite map_length length_gen_targs => k hk.
+    rewrite !nth_lookup.
+    f_equal.
+    rewrite list_lookup_fmap lookup_gen_targs_lt => //=.
+    rewrite -hlen in hk.
+    apply lookup_lt_is_Some_2 in hk.
+    destruct (targs !! k) => //=.
+    by elim hk.
+Qed.
+
+Lemma subst_mdef_gen_targs n mdef :
+  mdef_bounded n mdef →
+  subst_mdef (gen_targs n) mdef = mdef.
+Proof.
+  rewrite /mdef_bounded /subst_mdef; move => [/map_Forall_lookup hargs hret].
+  rewrite subst_ty_id => //.
+  replace (subst_ty (gen_targs n) <$> methodargs mdef) with (methodargs mdef);
+    first by destruct mdef.
+  apply map_eq => k.
+  rewrite lookup_fmap.
+  destruct (methodargs mdef !! k) as [ty | ] eqn:hty => //=.
+  apply hargs in hty.
+  by rewrite subst_ty_id.
+Qed.
+
+Lemma bounded_gen_targs n: Forall (bounded n) (gen_targs n).
+Proof.
+  rewrite Forall_forall => ty.
+  rewrite /gen_targs => h.
+  apply elem_of_list_fmap_2 in h as [ k [-> hk]].
+  constructor.
+  rewrite elem_of_seq /= in hk.
+  by destruct hk.
+Qed.
 
 (* A program is a collection of classes *)
 Class ProgDefContext := { Δ : stringmap classDef }.
 
 Section ProgDef.
-
   (* assume a given set of class definitions *)
   Context `{PDC: ProgDefContext}.
 
-  (* class A extends B *)
-  Definition extends (A B: tag) : Prop :=
-    ∃ cdef,
-    Δ !! A = Some cdef ∧
-    cdef.(superclass) = Some B
+  (* A type is well-formed w.r.t. Δ if all classes are
+   * defined in Δ, substitution applied to classes have the
+   * correct length, and they are all made of well-formed types.
+   *)
+  Inductive wf_ty : lang_ty → Prop :=
+    | WfInt : wf_ty IntT
+    | WfBool : wf_ty BoolT
+    | WfNothing : wf_ty NothingT
+    | WfMixed : wf_ty MixedT
+    | WfClassT t σ def:
+        Δ !! t = Some def →
+        length σ = def.(generics) →
+        (∀ k ty, σ !! k = Some ty → wf_ty ty) →
+        wf_ty (ClassT t σ)
+    | WfNull : wf_ty NullT
+    | WfNonNull : wf_ty NonNullT
+    | WfUnion s t : wf_ty s → wf_ty t → wf_ty (UnionT s t)
+    | WfInter s t : wf_ty s → wf_ty t → wf_ty (InterT s t)
+    | WfGen k: wf_ty (GenT k)
+    | WfEx t : wf_ty (ExT t)
   .
 
-  (* Refl trans closure of extends *)
-  Definition inherits := rtc extends.
+  Hint Constructors wf_ty : core.
 
-  (* Not useful, just for sanity check: inherits are chains.
-   * if A inherits B and C, then either B inherits C or C inherits B.
-   *)
-  Corollary inherits_is_chain:
-    ∀ A B C,
-    inherits A B → inherits A C →
-    (inherits C B ∨ inherits B C).
+  Lemma wf_ty_class_inv t σ:
+    wf_ty (ClassT t σ) →
+    Forall wf_ty σ.
   Proof.
-    intros A B C h; revert C.
-    induction h as [ t | x y z hxy hyz hi]; move => c hc; first by right.
-    destruct hxy as (cdef & hin & hs).
-    destruct hc as [ t | u v w huv hvw].
-    - left; econstructor; first by exists cdef. done.
-    - destruct huv as (? & hin' & hs').
-      rewrite hin' in hin.
-      injection hin; intros ->; clear hin hin'.
-      rewrite hs' in hs.
-      injection hs; intros ->; clear hs hs'.
-      apply hi in hvw as [h | h]; first by left.
-      by right.
+    move => h.
+    inv h.
+    apply Forall_forall => ty hin.
+    apply elem_of_list_lookup_1 in hin.
+    destruct hin as [k hk].
+    by apply H3 in hk.
   Qed.
 
+  Lemma wf_ty_subst σ ty :
+    Forall wf_ty σ →
+    wf_ty ty → wf_ty (subst_ty σ ty).
+  Proof.
+    move => hwf.
+    induction 1 as [ | | | | t targs def hdef hl h hi | | |
+        s t hs his ht hit | s t hs his ht hit | | ] => //=; try (by constructor).
+    - econstructor; [ done | by rewrite map_length | ].
+      move => k ty.
+      rewrite list_lookup_fmap.
+      destruct (targs !! k) as [ tk | ] eqn:htk => //=.
+      case => <-.
+      by eapply hi.
+    - destruct (σ !! k) as [ ty | ] eqn:hty => /=; last by constructor.
+      rewrite Forall_forall in hwf; apply hwf.
+      by apply elem_of_list_lookup_2 in hty.
+  Qed.
+
+  Lemma wf_ty_subst_map σ σ':
+    Forall wf_ty σ →
+    Forall wf_ty σ' →
+    Forall wf_ty (subst_ty σ <$> σ').
+  Proof.
+    move => h h'.
+    induction σ' as [ | hd tl hi ] => //=.
+    constructor.
+    - apply Forall_inv in h'.
+      by apply wf_ty_subst.
+    - apply hi.
+      by apply Forall_inv_tail in h'.
+  Qed.
+
+  Lemma gen_targs_wf n k ty: gen_targs n !! k = Some ty → wf_ty ty.
+  Proof.
+    rewrite /gen_targs -/fmap => hx.
+    apply list_lookup_fmap_inv in hx.
+    destruct hx as [ty' [ -> h]].
+    by constructor.
+  Qed.
+
+  (* A class definition 'parent' information is valid
+   * if the parent class actually exists, and the subsitution is:
+   * - of the right length (must capture all generics of the parent class)
+   * - bounded by the current class (must only mention generics of the current class)
+   * - be well-formed.
+   *)
+  Definition wf_cdef_parent (prog: stringmap classDef) cdef : Prop :=
+    match cdef.(superclass) with
+    | None => True
+    | Some (parent, σ) =>
+        ∃ pdef, prog !! parent = Some pdef ∧
+        length σ = pdef.(generics) ∧
+        Forall wf_ty σ ∧
+        Forall (bounded cdef.(generics)) σ
+    end
+  .
+  
+  Definition cdef_methods_bounded cdef : Prop :=
+    map_Forall (λ _mname mdef, mdef_bounded cdef.(generics) mdef) cdef.(classmethods).
+
+  (* source relation `class A<...> extends B<...>` *)
+  Inductive extends_using : tag → tag → list lang_ty → Prop :=
+    | ExtendsUsing A B cdef σB:
+        Δ !! A = Some cdef →
+        cdef.(superclass) = Some (B, σB) →
+        extends_using A B σB.
+
+  Hint Constructors extends_using : core.
+
+  Lemma extends_using_wf A B σ:
+    map_Forall (λ _cname, wf_cdef_parent Δ) Δ →
+    extends_using A B σ →
+    ∃ adef bdef,
+    Δ !! A = Some adef ∧
+    Δ !! B = Some bdef ∧
+    Forall (bounded adef.(generics)) σ ∧
+    length σ = bdef.(generics) ∧
+    Forall wf_ty σ.
+  Proof.
+    move => /map_Forall_lookup hwf hext.
+    inv hext.
+    assert (H' := H).
+    apply hwf in H.
+    rewrite /wf_cdef_parent H0 in H.
+    destruct H as (pdef & h & hlen & hσ & hf).
+    by exists cdef, pdef.
+  Qed.
+   
+  Inductive inherits_using : tag → tag → list lang_ty → Prop :=
+    | InheritsRefl A adef:
+        Δ !! A = Some adef →
+        inherits_using A A (gen_targs (adef.(generics)))
+    | InheritsExtends A B σ:
+        extends_using A B σ →
+        inherits_using A B σ
+    | InheritsTrans A B σB C σC:
+        extends_using A B σB →
+        inherits_using B C σC →
+        inherits_using A C (subst_ty σB <$> σC)
+  .
+
+  Hint Constructors inherits_using : core.
+
+  Lemma inherits_using_wf A B σ:
+    map_Forall (λ _cname, wf_cdef_parent Δ) Δ →
+    inherits_using A B σ →
+    ∃ adef bdef,
+    Δ !! A = Some adef ∧
+    Δ !! B = Some bdef ∧
+    Forall (bounded adef.(generics)) σ ∧
+    length σ = bdef.(generics) ∧
+    Forall wf_ty σ.
+  Proof.
+    move => hwf.
+    induction 1 as [ A adef hΔ | A B σ hext | A B σ C σC hext h hi ].
+    - exists adef, adef; repeat split => //.
+      + by apply bounded_gen_targs.
+      + by rewrite length_gen_targs.
+      + rewrite Forall_forall => x hx.
+        apply elem_of_list_lookup_1 in hx.
+        destruct hx as [i hi].
+        by apply gen_targs_wf in hi.
+    - by apply extends_using_wf.
+    - apply extends_using_wf in hext => //.
+      destruct hext as [adef [bdef [ha0 [hb0 [hf0 [hl0 hσ]]]]]].
+      destruct hi as [? [cdef [hb1 [hc1 [hf1 [hl1 hσC]]]]]].
+      simplify_eq.
+      exists adef, cdef; repeat split => //.
+      + rewrite Forall_forall => ty hin.
+        apply elem_of_list_fmap_2 in hin as [ty' [-> hin]].
+        rewrite Forall_forall in hf1; apply hf1 in hin.
+        by eapply bounded_subst.
+      + by rewrite map_length.
+      + apply Forall_forall => x hx.
+        apply elem_of_list_fmap_2 in hx as [ty [ -> hty]].
+        apply wf_ty_subst => //.
+        rewrite Forall_forall in hσC.
+        by apply hσC in hty.
+  Qed.
+
+  Lemma inherits_using_trans A B C σB σC:
+    map_Forall (λ _cname, wf_cdef_parent Δ) Δ →
+    inherits_using A B σB →
+    inherits_using B C σC →
+    inherits_using A C (subst_ty σB <$> σC).
+  Proof.
+    move => hwf h;
+    move : h C σC.
+    induction 1 as [ A cdef hΔ | A B s hext | A B s C t hext h hi] => Z σ' hin.
+    - rewrite subst_tys_id //.
+      apply inherits_using_wf in hin => //.
+      destruct hin as (? & ? & ? & ? & hF & _ ).
+      by simplify_eq.
+    - by econstructor.
+    - assert (hCZ := hin).
+      apply hi in hin; clear hi.
+      rewrite -map_subst_ty_subst; first by eapply InheritsTrans.
+      apply inherits_using_wf in h => //.
+      apply inherits_using_wf in hCZ => //.
+      destruct h as [bdef [cdef [hB [hC [hF0 [hlen0 _]]]]]].
+      destruct hCZ as [? [zdef [hC' [hZ [hF1 [hlen1 _]]]]]].
+      simplify_eq.
+      by rewrite hlen0.
+  Qed.
+
+  (* Stripped version of extends_using/inherits_using, mostly for
+   * evaluation when we don't care about the generics.
+   *) 
+  Inductive extends: tag → tag → Prop :=
+    | Extends A B cdef σB:
+        Δ !! A = Some cdef →
+        cdef.(superclass) = Some (B, σB) →
+        extends A B.
+
+  Hint Constructors extends : core.
+  Definition inherits := rtc extends.
+
+  (* Our class inheritance tree/forest doesn't have cycles. Which means
+   * inherits A B → inherits B A → A = B.
+   *)
+  Definition wf_no_cycle (prog: stringmap classDef) :=
+    ∀ A B σ σ', inherits_using A B σ → inherits_using B A σ' → A = B ∧ σ = σ'.
+
+  (* if A inherits B and A inherits C,
+   * then either B inherits C or C inherits B *)
+  Lemma inherits_using_chain A B σ:
+    map_Forall (λ _cname, wf_cdef_parent Δ) Δ →
+    inherits_using A B σ →
+    ∀ C σ', inherits_using A C σ' →
+    (∃ σ'', (subst_ty σ <$> σ'' = σ' ∧ inherits_using B C σ'') ∨
+            (subst_ty σ' <$> σ'' = σ ∧ inherits_using C B σ'')).
+  Proof.
+    move => hwf.
+    induction 1 as [ A adef hΔ | A B s hext | A B s C t hext h hi] => Z σ' hz.
+    - exists σ'; left; split => //.
+      apply subst_tys_id.
+      apply inherits_using_wf in hz => //.
+      destruct hz as (? & ? & ? & ? & hF & _ ).
+      by simplify_eq.
+    - inv hext; inv hz.
+      + simplify_eq.
+        exists s; right; split; last by econstructor; econstructor.
+        apply subst_tys_id.
+        apply hwf in H.
+        rewrite /wf_cdef_parent H0 in H.
+        by destruct H as (? & ? & _ & _ & hF).
+      + inv H1.
+        simplify_eq.
+        apply hwf in H.
+        rewrite /wf_cdef_parent H0 in H.
+        destruct H as (bdef & hB & hL & _ & hF).
+        exists (gen_targs bdef.(generics)); left; split; last by econstructor.
+        by rewrite subst_ty_gen_targs.
+      + inv H1.
+        simplify_eq.
+        exists σC; by left.
+    - destruct (inherits_using_wf _ _ _ hwf hz) as (adef & zdef & hA & hZ & hF0 & hL0 & _).
+      inv hext; inv hz.
+      + simplify_eq.
+        exists (subst_ty s <$> t); right; split; last first.
+        { eapply InheritsTrans => //.
+          by econstructor.
+        }
+        rewrite subst_tys_id // Forall_forall => ty hty.
+        apply elem_of_list_fmap_2 in hty as [ ty' [ -> hty']].
+        apply hwf in hA.
+        rewrite /wf_cdef_parent H0 in hA.
+        destruct hA as (bdef & hB & hL & _ & hF).
+        apply bounded_subst with (generics bdef) => //.
+        apply inherits_using_wf in h => //.
+        destruct h as (? & cdef & ? & hC & hF' & hL' & _); simplify_eq.
+        by rewrite Forall_forall in hF'; apply hF'.
+      + inv H1.
+        simplify_eq.
+        exists t; by right.
+      + inv H1.
+        simplify_eq.
+        apply hi in H2 as [σ'' [ [<- hx] | [<- hx]]]; clear hi.
+        * exists σ''; left; split; last done.
+          rewrite map_subst_ty_subst //.
+          apply inherits_using_wf in h => //.
+          apply inherits_using_wf in hx => //.
+          destruct h as (bdef & Cdef & ? & ? & hf0 & hl0 & _).
+          destruct hx as (? & zdef' & ? & ? & hf1 & hl1 & _).
+          simplify_eq.
+          by rewrite hl0.
+        * exists σ''; right; split; last done.
+          rewrite map_subst_ty_subst //.
+          apply inherits_using_wf in h => //.
+          apply inherits_using_wf in hx => //.
+          destruct h as (bdef & Cdef & ? & ? & hf0 & hl0 & _).
+          destruct hx as (zdef' & ? & ? & ? & hf1 & hl1 & _).
+          simplify_eq.
+          rewrite map_length in hL0.
+          by rewrite hL0.
+  Qed.
+
+  Lemma inherits_using_refl A σ:
+    wf_no_cycle Δ →
+    inherits_using A A σ →
+    ∃ adef, Δ !! A = Some adef ∧ σ = gen_targs adef.(generics).
+  Proof.
+    move => hwf hA.
+    assert (h: ∃ adef, Δ !! A = Some adef).
+    { inv hA.
+      - by exists adef.
+      - inv H.
+        by exists cdef.
+      - inv H.
+        by exists cdef.
+    }
+    destruct h as [adef hΔ].
+    exists adef; split => //.
+    eapply hwf; first by apply hA.
+    by constructor.
+  Qed.
+
+  Lemma inherits_using_fun A B σ:
+    wf_no_cycle Δ →
+    map_Forall (λ _cname, wf_cdef_parent Δ) Δ →
+    inherits_using A B σ →
+    ∀ σ', inherits_using A B σ' → σ = σ'.
+  Proof.
+    move => hwf hp.
+    induction 1 as [ A adef hΔ | A B s hext | A B s C t hext h hi ] => σ' hother.
+    - apply inherits_using_refl in hother as [? [h ->]] => //.
+      by simplify_eq.
+    - inv hext; inv hother.
+      + simplify_eq.
+        destruct (inherits_using_refl B s) as [? [h ->]] => //; last by simplify_eq.
+        eapply InheritsExtends.
+        by econstructor.
+      + inv H1; by simplify_eq.
+      + inv H1; simplify_eq.
+        apply inherits_using_refl in H2 as [bdef [hb ->]] => //.
+        rewrite subst_ty_gen_targs //.
+        apply hp in H.
+        rewrite /wf_cdef_parent H0 in H.
+        destruct H as [? [? [ -> _ ]]].
+        by simplify_eq.
+    - inv hext; inv hother.
+      + simplify_eq.
+        eapply hwf; last by constructor.
+        eapply InheritsTrans; last done.
+        by econstructor.
+      + inv H1; simplify_eq.
+        apply inherits_using_refl in h => //.
+        destruct h as [bdef [hB ->]].
+        rewrite subst_ty_gen_targs //.
+        apply hp in H.
+        rewrite /wf_cdef_parent H0 in H.
+        destruct H as [? [? [ -> _ ]]].
+        by simplify_eq.
+      + inv H1; simplify_eq.
+        apply hi in H2; by subst.
+  Qed.
+
+  (* Type well-formdness is mostly introduced to be able to define
+   * subtyping rule correctly, like unions.
+   *)
   Inductive subtype : lang_ty → lang_ty → Prop :=
     | SubMixed : ∀ ty, subtype ty MixedT
-    | SubClass : ∀ A B, inherits A B → subtype (ClassT A) (ClassT B)
+    | SubNothing : ∀ ty, wf_ty ty → subtype NothingT ty
+    | SubClass : ∀ A σA B σB adef,
+        Δ !! A = Some adef →
+        length σA = adef.(generics) →
+        extends_using A B σB →
+        subtype (ClassT A σA) (ClassT B (subst_ty σA <$> σB))
     | SubMixed2: subtype MixedT (UnionT NonNullT NullT)
     | SubIntNonNull: subtype IntT NonNullT
     | SubBoolNonNull: subtype BoolT NonNullT
-    | SubClassNonNull: ∀ A, subtype (ClassT A) NonNullT
-    | SubUnionUpper1 : ∀ s t, subtype s (UnionT s t)
-    | SubUnionUpper2 : ∀ s t, subtype t (UnionT s t)
+    | SubClassNonNull: ∀ A targs, subtype (ClassT A targs) NonNullT
+    | SubUnionUpper1 : ∀ s t, wf_ty t → subtype s (UnionT s t)
+    | SubUnionUpper2 : ∀ s t, wf_ty s → subtype t (UnionT s t)
         (* TODO: Do we need this one ? *)
     | SubUnionLeast : ∀ s t u, subtype s u → subtype t u → subtype (UnionT s t) u
     | SubInterLower1 : ∀ s t, subtype (InterT s t) s
@@ -145,535 +780,1330 @@ Section ProgDef.
     | SubInterGreatest: ∀ s t u, subtype u s → subtype u t → subtype u (InterT s t)
     | SubRefl: ∀ s, subtype s s
     | SubTrans : ∀ s t u, subtype s t → subtype t u → subtype s u
-    .
+  .
 
-    Hint Constructors subtype : core.
+  Hint Constructors subtype : core.
 
-    Notation "s <: t" := (subtype s t) (at level 70, no associativity).
+  Notation "s <: t" := (subtype s t) (at level 70, no associativity).
 
-    (* Derived rules *)
-    Lemma subtype_union_comm : ∀ A B, (UnionT A B) <: (UnionT B A).
-    Proof. by auto.  Qed.
+  Lemma subtype_wf A B:
+    map_Forall (λ _cname, wf_cdef_parent Δ) Δ →
+    wf_ty A → A <: B → wf_ty B.
+  Proof.
+    move => hp hwf.
+    induction 1 as [ ty | ty h | A σA B σB adef hΔ hA hext | | | | A args | s t h
+      | s t h | s t u hs his ht hit | s t | s t | s t u hs his ht hit | s
+      | s t u hst hist htu hitu ] => //=; try (by constructor).
+    - inv hext; simplify_eq.
+      rewrite /map_Forall_lookup in hp.
+      apply hp in hΔ.
+      rewrite /wf_cdef_parent H0 in hΔ.
+      destruct hΔ as (bdef & hB & hL & hσB & hb).
+      econstructor; first done.
+      + by rewrite map_length.
+      + move => k ty.
+        rewrite list_lookup_fmap.
+        destruct (σB !! k) as [ tyk | ] eqn:hty => //=.
+        case => <-.
+        apply wf_ty_subst; first by apply wf_ty_class_inv in hwf.
+        rewrite Forall_forall in hσB.
+        apply elem_of_list_lookup_2 in hty.
+        by apply hσB in hty.
+    - inv hwf; by eauto.
+    - inv hwf; by eauto.
+    - inv hwf; by eauto.
+    - constructor; by eauto.
+    - by eauto.
+  Qed.
 
-    Lemma subtype_inter_comm : ∀ A B, (InterT A B) <: (InterT B A).
-    Proof. by auto.  Qed.
+  Lemma subtype_subst A B:
+    map_Forall (λ _cname, wf_cdef_parent Δ) Δ →
+    A <: B → ∀ σ,
+    Forall wf_ty σ →
+    (subst_ty σ A) <: (subst_ty σ B).
+  Proof.
+    move => hp.
+    induction 1 as [ ty | ty h | A σA B σB adef hΔ hA hext | | | | A args | s t h
+      | s t h | s t u hs his ht hit | s t | s t | s t u hs his ht hit | s
+      | s t u hst hist htu hitu ] => σ hσ //=.
+    - constructor.
+      by apply wf_ty_subst.
+    - rewrite map_subst_ty_subst.
+      + econstructor => //.
+        by rewrite map_length.
+      + apply extends_using_wf in hext => //.
+      destruct hext as (? & bdef & ? & hB & hF & hL).
+      simplify_eq.
+      by rewrite hA.
+    - constructor.
+      by apply wf_ty_subst.
+    - constructor.
+      by apply wf_ty_subst.
+    - constructor; by eauto.
+    - econstructor; by eauto.
+    - econstructor; by eauto.
+  Qed.
 
-    Lemma subtype_union_assoc:
-      ∀ A B C, (UnionT (UnionT A B) C) <: (UnionT A (UnionT B C)).
-    Proof. by eauto.  Qed.
+  (* Sanity checks: Some derived rules *)
+  Lemma subtype_union_comm : ∀ A B,
+    wf_ty A → wf_ty B →
+    (UnionT A B) <: (UnionT B A).
+  Proof. by auto. Qed.
 
-    Lemma subtype_inter_assoc:
-      ∀ A B C, (InterT (InterT A B) C) <: (InterT A (InterT B C)).
-    Proof. by eauto.  Qed.
+  Lemma subtype_inter_comm : ∀ A B,
+    wf_ty A → wf_ty B →
+    (InterT A B) <: (InterT B A).
+  Proof. by auto. Qed.
 
-    Definition local_tys := stringmap lang_ty.
+  Lemma subtype_union_assoc:
+    ∀ A B C,
+    wf_ty A → wf_ty B → wf_ty C →
+    (UnionT (UnionT A B) C) <: (UnionT A (UnionT B C)).
+  Proof.
+    move => A B C wfA wfB wfC.
+    apply SubUnionLeast; last by eauto.
+    apply SubUnionLeast; last by eauto.
+    apply SubUnionUpper1.
+    constructor; by eauto.
+  Qed.
 
-    Definition lty_sub (lty rty: local_tys) :=
-      ∀ k A, rty !! k = Some A → ∃ B, lty !! k = Some B ∧ B <: A.
+  Lemma subtype_inter_assoc:
+    ∀ A B C, 
+    wf_ty A → wf_ty B → wf_ty C →
+    (InterT (InterT A B) C) <: (InterT A (InterT B C)).
+  Proof. by eauto. Qed.
 
-    Notation "lty <:< rty" := (lty_sub lty rty) (at level 70, no associativity).
+  (* Generalized version of SubClass to any inheritance sequence *)
+  Lemma subtype_inherits_using A B σ σA adef:
+    map_Forall (λ _ : string, wf_cdef_parent Δ) Δ →
+    Δ !! A = Some adef →
+    length σA = adef.(generics) →
+    inherits_using A B σ →
+    ClassT A σA <: ClassT B (subst_ty σA <$> σ).
+  Proof.
+    move => hp hA hl h.
+    move : h σA adef hA hl.
+    induction 1 as [ A ? h | A B σ0 hext | A B σ0 C σC hext h hi ] => σA ? hA hl.
+    - simplify_eq.
+      by rewrite subst_ty_gen_targs.
+    - by econstructor.
+    - eapply SubTrans; first by eapply SubClass.
+      apply extends_using_wf in hext => //.
+      destruct hext as (? & bdef & hadef' & hbdef & hF0 & hL0 & _).
+      apply inherits_using_wf in h => //.
+      destruct h as (? & cdef & hbdef' & hcdef & hF1 & hL1 & _).
+      simplify_eq.
+      rewrite map_subst_ty_subst; last by rewrite hL0.
+      apply hi with bdef => //.
+      by rewrite map_length.
+  Qed.
 
-    Lemma lty_sub_reflexive: reflexive _ lty_sub.
-    Proof.
-      move => lty k A ->.
-      by exists A.
-    Qed.
+  (* Typing contexts *)
+  Definition local_tys := stringmap lang_ty.
 
-    Lemma lty_sub_transitive: transitive _ lty_sub.
-    Proof.
-      move => lty rty zty hlr hrz k A hA.
-      apply hrz in hA as (C & hC & hsub).
-      apply hlr in hC as (B & -> & hsub').
-      exists B; by eauto.
-    Qed.
+  (* Subtype / Inclusion of typing contexts *)
+  Definition lty_sub (lty rty: local_tys) :=
+    ∀ k A, rty !! k = Some A → ∃ B, lty !! k = Some B ∧ B <: A.
 
-    (* has_field fname ty cname checks if the class cname has a field named
-     * fname of type ty
-     *)
-    Inductive has_field (fname: string) (typ: lang_ty): tag → Prop :=
-      | HasField current cdef:
-          Δ !! current = Some cdef →
-          cdef.(classfields) !! fname = Some typ →
-          has_field fname typ current
-      | InheritsField current parent cdef:
-          Δ !! current = Some cdef →
-          cdef.(classfields) !! fname = None →
-          cdef.(superclass) = Some parent →
-          has_field fname typ parent →
-          has_field fname typ current.
+  Notation "lty <:< rty" := (lty_sub lty rty) (at level 70, no associativity).
 
-    Hint Constructors has_field : core.
+  Lemma lty_sub_reflexive: reflexive _ lty_sub.
+  Proof.
+    move => lty k A ->.
+    by exists A.
+  Qed.
 
-    (* Naive method lookup: methods are unique *)
-    Inductive has_method (mname: string) (mdef: methodDef): tag → Prop :=
-      | HasMethod current cdef:
-          Δ !! current = Some cdef →
-          cdef.(classmethods) !! mname = Some mdef →
-          has_method mname mdef current
-      | InheritsMethod current parent cdef:
-          Δ !! current = Some cdef →
-          cdef.(classmethods) !! mname = None →
-          cdef.(superclass) = Some parent →
-          has_method mname mdef parent →
-          has_method mname mdef current
-    .
+  Lemma lty_sub_transitive: transitive _ lty_sub.
+  Proof.
+    move => lty rty zty hlr hrz k A hA.
+    apply hrz in hA as (C & hC & hsub).
+    apply hlr in hC as (B & -> & hsub').
+    exists B; by eauto.
+  Qed.
 
-    Hint Constructors has_method : code.
+  Lemma lty_sub_insert_1 lhs ty lty0 lty1:
+    lty0 <:< lty1 →
+    <[lhs:=ty]> lty0 <:< <[lhs:=ty]> lty1.
+  Proof.
+    move => h x xty.
+    rewrite lookup_insert_Some.
+    case => [[<- <-] | [hne hin]].
+    - rewrite lookup_insert; by exists ty.
+    - rewrite lookup_insert_ne //.
+      apply h in hin.
+      destruct hin as [B [hin hsub]].
+      by exists B.
+  Qed.
 
-    Lemma has_method_from m mdef A:
-      has_method m mdef A →
-      ∃ B cdef,
-      Δ !! B = Some cdef ∧
-      cdef.(classmethods) !! m = Some mdef ∧
-      inherits A B.
-    Proof.
-      induction 1 as [ current cdef hΔ hm | current parent cdef hΔ hm hs h hi];
-          first by exists current, cdef.
-      destruct hi as (B & cdef' & hΔ' & hm' & hinherits). 
-      exists B, cdef'; repeat split => //.
-      econstructor; last by apply hinherits.
-      by exists cdef.
-    Qed.
+  Lemma lty_sub_insert_2 ty0 ty1 lhs lty:
+    ty0 <: ty1 →
+    <[lhs := ty0]>lty <:< <[lhs := ty1]> lty.
+  Proof.
+    move => hsub k ty.
+    rewrite lookup_insert_Some.
+    case => [[<- <-] | [hne hin]].
+    - exists ty0; by rewrite lookup_insert.
+    - exists ty; by rewrite lookup_insert_ne.
+  Qed.
 
-    (* A class cannot redeclare a field if it is present in
-     * any of its parent definition.
-     *)
-    Definition wf_cdef_fields cdef : Prop :=
-      ∀ f fty super,
-      cdef.(superclass) = Some super →
-      has_field f fty super →
-      cdef.(classfields) !! f = None.
+  Lemma lty_sub_subst σ lty rty:
+    map_Forall (λ _ : string, wf_cdef_parent Δ) Δ →
+    Forall wf_ty σ →
+    lty <:< rty → (subst_ty σ <$> lty) <:< (subst_ty σ <$> rty).
+  Proof.
+    move => hp hσ hsub k A.
+    rewrite lookup_fmap_Some.
+    case => B [<- hk].
+    apply hsub in hk as [ B' [HB' hsub']].
+    exists (subst_ty σ B').
+    rewrite lookup_fmap HB'; split; first done.
+    by apply subtype_subst.
+  Qed.
 
-    (* We allow method override: children can redeclare a method if types
-     * are compatible:
-     * - return type must be a subtype
-     * - argument types must be a supertype
-     *)
-    Definition mdef_incl sub super :=
-      dom stringset sub.(methodargs) = dom _ super.(methodargs) ∧
-      (∀ k A B, sub.(methodargs) !! k = Some A →
-      super.(methodargs) !! k = Some B → B <: A) ∧
-      sub.(methodrettype) <: super.(methodrettype).
+  (* has_field f C fty means that class C defines or inherits a field f
+   * of type fty. The type is substituted accordingly so it can be
+   * interpreted in C directly.
+   *)
+  Inductive has_field (fname: string) : tag -> lang_ty → Prop :=
+    | HasField tag cdef typ:
+        Δ !! tag = Some cdef →
+        cdef.(classfields) !! fname = Some typ →
+        has_field fname tag typ
+    | InheritsField tag targs parent cdef typ:
+        Δ !! tag = Some cdef →
+        cdef.(classfields) !! fname = None →
+        cdef.(superclass) = Some (parent, targs) →
+        has_field fname parent typ →
+        has_field fname tag (subst_ty targs typ)
+  .
 
-    Lemma mdef_incl_reflexive: reflexive _ mdef_incl.
-    Proof.
-      move => mdef; split; first done.
-      split; last done.
-      by move => k A B -> [] ->.
-    Qed.
+  Hint Constructors has_field : core.
 
-    Lemma mdef_incl_transitive: transitive _ mdef_incl.
-    Proof.
-      move => m0 m1 m2 [hdom1 [h1 ?]] [hdom2 [h2 ?]]; split; first by etransitivity.
-      split; last by eauto.
-      move => k A B hA hB.
-      destruct (methodargs m1 !! k) as [C | ] eqn:hC; last first.
-      { apply mk_is_Some in hA.
-        apply elem_of_dom in hA.
-        rewrite hdom1 in hA.
-        apply elem_of_dom in hA.
-        rewrite hC in hA.
-        by elim: hA.
+  (* has_field is a functional relation *)
+  Lemma has_field_fun fname A typ:
+    has_field fname A typ →
+    ∀ typ', has_field fname A typ' →
+    typ = typ'.
+  Proof.
+    induction 1 as [ tag cdef typ hΔ hf
+      | tag targs parent cdef typ hΔ hf hs h hi ] => typ' h'.
+    - inv h'; by simplify_eq.
+    - inv h'.
+      + by simplify_eq.
+      + simplify_eq.
+        by rewrite (hi _ H2).
+  Qed.
+
+  (* A class cannot redeclare a field if it is already present in
+   * any of its parent definition.
+   * (No field override)
+   *)
+  Definition wf_cdef_fields cdef : Prop :=
+    ∀ f fty super inst,
+    cdef.(superclass) = Some (super, inst) →
+    has_field f super fty →
+    cdef.(classfields) !! f = None.
+
+  (* All field types in a class must be bounded by the class generics *)
+  Definition wf_cdef_fields_bounded cdef : Prop :=
+    map_Forall (λ _fname, bounded cdef.(generics)) cdef.(classfields).
+
+  (* All field types in a class must be well-formed *)
+  Definition wf_cdef_fields_wf cdef : Prop :=
+    map_Forall (λ _fname, wf_ty) cdef.(classfields). 
+
+  Lemma has_field_wf f t fty :
+    map_Forall (λ _cname, wf_cdef_parent Δ) Δ →
+    map_Forall (λ _, wf_cdef_fields_wf) Δ →
+    has_field f t fty →
+    wf_ty fty.
+  Proof.
+    move => /map_Forall_lookup hp /map_Forall_lookup hwf.
+    induction 1 as [ tag cdef typ hΔ hf
+      | tag targs parent cdef typ hΔ hf hs h hi ].
+    - apply hwf in hΔ.
+      by apply hΔ in hf.
+    - apply wf_ty_subst => //.
+      apply hp in hΔ.
+      rewrite /wf_cdef_parent hs in hΔ.
+      by destruct hΔ as (pdef & ? & ? & htargs & _).
+  Qed.
+
+  (* If a class has a field f, then any subclass will inherit it,
+   * with the right substituted type.
+   *)
+  Lemma has_field_extends_using f B typ:
+    map_Forall (λ _cname, wf_cdef_fields) Δ →
+    has_field f B typ →
+    ∀ A σB,
+    extends_using A B σB →
+    has_field f A (subst_ty σB typ).
+  Proof.
+    move => hwf hf A σB hext.
+    rewrite map_Forall_lookup in hwf.
+    inv hext.
+    eapply InheritsField => //.
+    by eapply hwf.
+  Qed.
+
+  Lemma has_field_bounded f t fty:
+    map_Forall (λ _cname, wf_cdef_parent Δ) Δ →
+    map_Forall (λ _cname, wf_cdef_fields_bounded) Δ →
+    has_field f t fty →
+    ∃ def, Δ !! t = Some def ∧ bounded def.(generics) fty.
+  Proof.
+    move => /map_Forall_lookup hwfparent /map_Forall_lookup hwfb.
+    induction 1 as [ tag cdef typ hΔ hf
+      | tag targs parent cdef typ hΔ hf hs h hi ].
+    - exists cdef; split => //.
+      apply hwfb in hΔ.
+      by apply hΔ in hf.
+    - exists cdef; split => //.
+      destruct hi as [pdef [ hp hb]].
+      apply hwfparent in hΔ.
+      rewrite /wf_cdef_parent hs hp in hΔ.
+      destruct hΔ as (? & [= <-] & h0 & _ & h1).
+      by eapply bounded_subst.
+  Qed.
+
+  (* like has_field_extends_using, for any chain of inheritance. *)
+  Lemma has_field_inherits_using f B typ:
+    map_Forall (λ _cname, wf_cdef_parent Δ) Δ →
+    map_Forall (λ _cname, wf_cdef_fields) Δ →
+    map_Forall (λ _cname, wf_cdef_fields_bounded) Δ →
+    has_field f B typ →
+    ∀ A σB,
+    inherits_using A B σB →
+    has_field f A (subst_ty σB typ).
+  Proof.
+    move => hp hfs hfb hf A σB hin.
+    induction hin as [ A adef | A B σ hext | A B σ C σC hext h hi].
+    - rewrite subst_ty_id //.
+      apply has_field_bounded in hf => //.
+      destruct hf as [? [? h]].
+      by simplify_eq.
+    - by eapply has_field_extends_using.
+    - destruct (has_field_bounded _ _ _ hp hfb hf) as (cdef & hcdef & hc).
+      apply hi in hf; clear hi.
+      apply has_field_extends_using with (A := A) (σB := σ) in hf => //.
+      rewrite -subst_ty_subst //.
+      apply inherits_using_wf in h => //.
+      destruct h as (? & ? & ? & ? & ? & h & _).
+      simplify_eq.
+      by rewrite h.
+  Qed.
+
+  (* Helper predicate to collect all fields of a given class, as a map *)
+  Definition has_fields A (fields: stringmap lang_ty) : Prop :=
+    ∀ fname typ, has_field fname A typ ↔ fields !! fname = Some typ.
+
+  (* has_method m C orig mdef means that class C inherits a method m,
+   * described by the methodDef mdef.
+   *
+   * The method is declared in class orig (which can be C).
+   * mdef is substituted accordingly to be interpreted in the class C.
+   * 
+   * Note that we do support method override (see mdef_incl below).
+   *)
+  Inductive has_method (mname: string) : tag → tag → methodDef → Prop :=
+    | HasMethod tag cdef mdef:
+        Δ !! tag = Some cdef →
+        cdef.(classmethods) !! mname = Some mdef →
+        has_method mname tag tag mdef
+    | InheritsMethod tag parent orig σ cdef mdef:
+        Δ !! tag = Some cdef →
+        cdef.(classmethods) !! mname = None →
+        cdef.(superclass) = Some (parent, σ) →
+        has_method mname parent orig mdef →
+        has_method mname tag orig (subst_mdef σ mdef)
+  .
+
+  Hint Constructors has_method : code.
+
+  (* a method is well-formed if the type of all its arguments, and its
+   * return type are well-formed.
+   *)
+  Definition mdef_wf mdef : Prop :=
+    map_Forall (λ _mname, wf_ty) mdef.(methodargs) ∧
+    wf_ty mdef.(methodrettype).
+
+  (* all method of a class are well-formed *)
+  Definition wf_cdef_methods_wf cdef : Prop :=
+    map_Forall (λ _mname, mdef_wf) cdef.(classmethods).
+
+  Lemma has_method_wf m t orig mdef:
+    map_Forall (λ _cname, wf_cdef_parent Δ) Δ →
+    map_Forall (λ _, wf_cdef_methods_wf) Δ →
+    has_method m t orig mdef →
+    map_Forall (λ _mname, wf_ty) mdef.(methodargs) ∧
+    wf_ty mdef.(methodrettype).
+  Proof.
+    move => hp hm.
+    induction 1 as [ tag cdef mdef ht hin |
+        tag parent orig σ cdef mdef ht hin hs h [hia hir] ].
+    - apply hm in ht.
+      by apply ht in hin.
+    - assert (hσ : Forall wf_ty σ).
+      { rewrite map_Forall_lookup in hp.
+        apply hp in ht.
+        rewrite /wf_cdef_parent hs in ht.
+        by destruct ht as (? & ? & ? & ? & ?).
       }
-      apply SubTrans with C.
-      - by eapply h2.
-      - by eapply h1.
-    Qed.
+      split.
+      + apply map_Forall_lookup => k ty.
+        rewrite lookup_fmap_Some.
+        case => ty' [<- hk].
+        apply wf_ty_subst => //.
+        rewrite map_Forall_lookup in hia.
+        by apply hia in hk.
+      + rewrite /subst_mdef /=.
+        by apply wf_ty_subst.
+  Qed.
 
-    Definition wf_cdef_methods cdef : Prop :=
-      ∀ m mdef superdef super,
-      cdef.(superclass) = Some super →
-      has_method m superdef super →
-      cdef.(classmethods) !! m = Some mdef →
-      mdef_incl mdef superdef.
+  (* We allow method override: children can redeclare a method if types
+   * are compatible:
+   * - return type must be a subtype
+   * - argument types must be a supertype
+   *)
+  Definition mdef_incl sub super :=
+    dom stringset sub.(methodargs) = dom _ super.(methodargs) ∧
+    (∀ k A B, sub.(methodargs) !! k = Some A →
+    super.(methodargs) !! k = Some B → B <: A) ∧
+    sub.(methodrettype) <: super.(methodrettype).
 
-    (* all fields of class cname are in the fnames set *)
-    Definition has_fields (cname: tag) (fnames: stringmap lang_ty) : Prop :=
-      ∀ fname typ, has_field fname typ cname ↔ fnames !! fname = Some typ.
+  Lemma mdef_incl_reflexive: reflexive _ mdef_incl.
+  Proof.
+    move => mdef; split; first done.
+    split; last done.
+    by move => k A B -> [] ->.
+  Qed.
 
-    Lemma has_fields_fun: ∀ c fs0 fs1,
-      has_fields c fs0 → has_fields c fs1 → fs0 = fs1.
-    Proof.
-      move => c fs0 fs1 h0 h1.
-      apply map_eq => k.
-      destruct (fs0 !! k) as [ ty | ] eqn:hty.
-      - destruct (h1 k ty) as [hl1 hr1].
-        rewrite hl1 //=.
-        by apply h0.
-      - destruct (fs1 !! k) as [ ty | ] eqn:hty'; last done.
-        destruct (h1 k ty) as [hl1 hr1].
-        apply h0 in hr1; last done.
-        by rewrite hty in hr1.
-    Qed.
-
-    Lemma has_method_fun: ∀ c name mdef0 mdef1,
-      has_method name mdef0 c → has_method name mdef1 c → mdef0 = mdef1.
-    Proof.
-      move => c name mdef0 mdef1 h; move: mdef1.
-      induction h as [ current cdef hΔ hm | current parent cdef hΔ hm hs hp hi ].
-      - move => mdef1 h1; inv h1.
-        + rewrite hΔ in H; injection H; intros; subst; clear hΔ H.
-          rewrite hm in H0; by injection H0.
-        + rewrite hΔ in H; injection H; intros; subst; clear hΔ H.
-          rewrite hm in H0; discriminate H0.
-      - move => mdef1 h1; inv h1.
-        + rewrite hΔ in H; injection H; intros; subst; clear hΔ H.
-          rewrite hm in H0; discriminate H0.
-        + rewrite hΔ in H; injection H; intros; subst; clear hΔ H.
-          rewrite hs in H1; injection H1; intros; subst; clear hs H1.
-          by apply hi.
-    Qed.
-
-    Lemma has_field_inherits : map_Forall (fun _ => wf_cdef_fields) Δ →
-      ∀ A B, inherits A B →
-      ∀ f fty, has_field f fty B → has_field f fty A.
-    Proof.
-      move => wfΔ A B h.
-      induction h as [ t | x y z hxy hyz hi]; move => f fty hf; first done.
-      apply hi in hf.
-      destruct hxy as (cdef & hΔ & hs).
-      apply InheritsField with y cdef; move => //.
-      apply wfΔ in hΔ.
-      by eapply hΔ.
-    Qed.
-
-    Corollary has_fields_inherits_lookup:
-      map_Forall (fun _ => wf_cdef_fields) Δ →
-      ∀ A B name fty fields,
-      has_field name fty B →
-      inherits A B →
-      has_fields A fields →
-      fields !! name = Some fty.
-    Proof.
-      move => wfΔ A B name fty fields hfields hinherits hf.
-      destruct (hf name fty) as [hl hr].
-      apply hl.
-      by eapply (has_field_inherits wfΔ).
-    Qed.
-
-    Lemma has_method_inherits (Hcdef: map_Forall (fun _ => wf_cdef_methods) Δ):
-      ∀ A B, inherits A B →
-      ∀ m mdef, has_method m mdef B →
-      ∃ mdef', has_method m mdef' A ∧ mdef_incl mdef' mdef.
-    Proof.
-      move => A B h.
-      induction h as [ t | x y z hxy hyz hi]; move => m mdef hf.
-      { exists mdef; split => //.
-        by apply mdef_incl_reflexive.
-      }
-      apply hi in hf as (mdef' & hm & hincl).
-      destruct hxy as (cdef & hΔ & hs).
-      destruct (cdef.(classmethods) !! m) as [ mdef'' | ] eqn:heq; last first.
-      { exists mdef'; split; last done.
-        by apply InheritsMethod with y cdef.
-      }
-      exists mdef''; split; first by apply HasMethod with cdef.
-      apply mdef_incl_transitive with mdef'; last done.
-      apply Hcdef in hΔ.
-      by eapply hΔ.
-    Qed.
-
-    (* Typing Judgements *)
-    Definition is_bool_op op : bool :=
-      match op with
-      | LeqO | GeqO | EqO => true
-      | PlusO | MinusO | TimesO | DivO => false
-      end
-    .
-
-    Inductive expr_has_ty (lty : local_tys) :
-      expr → lang_ty → Prop :=
-      | IntTy : ∀ z, expr_has_ty lty (IntE z) IntT
-      | BoolTy: ∀ b, expr_has_ty lty (BoolE b) BoolT
-      | NullTy: expr_has_ty lty NullE NullT
-      | OpIntTy: ∀ op e1 e2,
-          is_bool_op op = false →
-          expr_has_ty lty e1 IntT →
-          expr_has_ty lty e2 IntT →
-          expr_has_ty lty (OpE op e1 e2) IntT
-      | OpBoolTy: ∀ op e1 e2,
-          is_bool_op op = true →
-          expr_has_ty lty e1 IntT →
-          expr_has_ty lty e2 IntT →
-          expr_has_ty lty (OpE op e1 e2) BoolT
-      | VarTy: ∀ v ty,
-          lty !! v = Some ty →
-          expr_has_ty lty (VarE v) ty
-      | ESubTy: ∀ e s t,
-          expr_has_ty lty e s →
-          s <: t →
-          expr_has_ty lty e t
-    .
-
-    (* continuation-based typing for commands *)
-    Inductive cmd_has_ty :
-      local_tys → cmd → local_tys → Prop :=
-      | SkipTy: ∀ lty, cmd_has_ty lty SkipC lty
-      | SeqTy: ∀ lty1 lty2 lty3 fstc sndc,
-          cmd_has_ty lty1 fstc lty2 →
-          cmd_has_ty lty2 sndc lty3 →
-          cmd_has_ty lty1 (SeqC fstc sndc) lty3
-      | LetTy: ∀ lty lhs e ty,
-          expr_has_ty lty e ty →
-          cmd_has_ty lty (LetC lhs e) (<[lhs := ty]>lty)
-      | IfTy: ∀ lty1 lty2 cond thn els,
-          expr_has_ty lty1 cond BoolT →
-          cmd_has_ty lty1 thn lty2 →
-          cmd_has_ty lty1 els lty2 →
-          cmd_has_ty lty1 (IfC cond thn els) lty2
-      | GetTy: ∀ lty lhs recv t name fty,
-          expr_has_ty lty recv (ClassT t) →
-          has_field name fty t →
-          cmd_has_ty lty (GetC lhs recv name) (<[lhs := fty]>lty)
-      | SetTy: ∀ lty recv fld rhs fty t,
-          expr_has_ty lty recv (ClassT t) →
-          expr_has_ty lty rhs fty →
-          has_field fld fty t →
-          cmd_has_ty lty (SetC recv fld rhs) lty
-      | NewTy: ∀ lty lhs t args fields,
-          has_fields t fields →
-          dom (gset string) fields = dom _ args →
-          (∀ f fty arg,
-          fields !! f = Some fty →
-          args !! f = Some arg →
-          expr_has_ty lty arg fty) →
-          cmd_has_ty lty (NewC lhs t args) (<[ lhs := ClassT t]>lty)
-      | CallTy: ∀ lty lhs recv t name mdef args,
-          expr_has_ty lty recv (ClassT t) →
-          has_method name mdef t →
-          dom (gset string) mdef.(methodargs) = dom _ args →
-          (∀ x ty arg,
-          mdef.(methodargs) !! x = Some ty →
-          args !! x = Some arg →
-          expr_has_ty lty arg ty) →
-          cmd_has_ty lty (CallC lhs recv name args) (<[lhs := mdef.(methodrettype)]>lty)
-      | SubTy: ∀ lty c rty rty',
-          rty' <:< rty →
-          cmd_has_ty lty c rty' →
-          cmd_has_ty lty c rty
-      | CondTagTy lty v tv t cmd :
-          lty !! v = Some tv →
-          cmd_has_ty (<[v:=InterT tv (ClassT t)]> lty) cmd lty →
-          cmd_has_ty lty (CondTagC v t cmd) lty
-    .
-
-    Corollary CallTy_: ∀ lty lhs recv t name mdef args,
-      expr_has_ty lty recv (ClassT t) →
-      has_method name mdef t →
-      dom (gset string) mdef.(methodargs) = dom _ args →
-      (∀ x ty arg,
-      mdef.(methodargs) !! x = Some ty →
-      args !! x = Some arg →
-      ∃ ty', ty' <: ty ∧ expr_has_ty lty arg ty') →
-      cmd_has_ty lty (CallC lhs recv name args) (<[lhs := mdef.(methodrettype)]>lty).
-    Proof.
-      move => lty lhs recv t name mdef args hrecv hmdef hdom hargs.
-      econstructor; [done | done | done | ].
-      move => k ty arg hk ha.
-      destruct (hargs _ _ _ hk ha) as (ty' & hsub & he).
-      by econstructor.
-    Qed.
-
-    Lemma CallTyGen: ∀ lty lhs recv t name mdef args ret,
-      expr_has_ty lty recv (ClassT t) →
-      has_method name mdef t →
-      dom (gset string) mdef.(methodargs) = dom _ args →
-      (∀ x ty arg,
-      mdef.(methodargs) !! x = Some ty →
-      args !! x = Some arg →
-      ∃ ty', ty' <: ty ∧ expr_has_ty lty arg ty') →
-      mdef.(methodrettype) <: ret →
-      cmd_has_ty lty (CallC lhs recv name args) (<[lhs := ret]>lty).
-    Proof.
-      move =>lty lhs ????? ret hrecv hm hdom hargs hret.
-      eapply SubTy; last by eapply CallTy_.
-      move => k A hA.
-      rewrite lookup_insert_Some in hA.
-      destruct hA as [[<- <-] | [hne heq]].
-      - rewrite lookup_insert.
-        by eexists.
-      - rewrite lookup_insert_ne //.
-        by exists A.
-    Qed.
-
-    Definition wf_mdef_ty t mdef :=
-      ∃ lty,
-      cmd_has_ty (<["$this" := ClassT t]>mdef.(methodargs)) mdef.(methodbody) lty ∧
-      expr_has_ty lty mdef.(methodret) mdef.(methodrettype)
-    .
-
-    Record wf_cdefs (prog: stringmap classDef)  := {
-      wf_fields : map_Forall (fun cname => wf_cdef_fields) prog;
-      wf_methods : map_Forall (fun cname => wf_cdef_methods) prog;
-      wf_mdefs :
-      map_Forall (fun cname cdef =>
-      map_Forall (fun mname mdef => wf_mdef_ty cname mdef) cdef.(classmethods)) prog
+  Lemma mdef_incl_transitive: transitive _ mdef_incl.
+  Proof.
+    move => m0 m1 m2 [hdom1 [h1 ?]] [hdom2 [h2 ?]]; split; first by etransitivity.
+    split; last by eauto.
+    move => k A B hA hB.
+    destruct (methodargs m1 !! k) as [C | ] eqn:hC; last first.
+    { apply mk_is_Some in hA.
+      apply elem_of_dom in hA.
+      rewrite hdom1 in hA.
+      apply elem_of_dom in hA.
+      rewrite hC in hA.
+      by elim: hA.
     }
-    .
+    apply SubTrans with C.
+    - by eapply h2.
+    - by eapply h1.
+  Qed.
 
-    (* Big set reduction *)
-    Definition primop_eval (op: primop) : Z → Z → value :=
-      match op with
-      | PlusO => fun x y => IntV (x + y)
-      | MinusO => fun x y => IntV (x - y)
-      | TimesO => fun x y => IntV (x * y)
-      | DivO => fun x y => IntV (x / y)
-      | LeqO => fun x y => BoolV (Z.leb x y)
-      | GeqO => fun x y => BoolV (Z.geb x y)
-      | EqO => fun x y => BoolV (Z.eqb x y)
-      end
-    .
+  Lemma mdef_incl_subst mdef0 mdef1 σ :
+    map_Forall (λ _cname, wf_cdef_parent Δ) Δ →
+    Forall wf_ty σ →
+    mdef_incl mdef0 mdef1 →
+    mdef_incl (subst_mdef σ mdef0) (subst_mdef σ mdef1).
+  Proof.
+    move => hp hσ.
+    rewrite /mdef_incl /subst_mdef /=.
+    case => [hdom [hargs hret]]; split; first by rewrite !dom_fmap_L.
+    split; last by apply subtype_subst.
+    move => k A B.
+    rewrite !lookup_fmap_Some.
+    case => tyA [<- hA].
+    case => tyB [<- hB].
+    apply subtype_subst => //.
+    by eapply hargs.
+  Qed.
 
-    Definition local_env := gmap var value.
+  (* has_method is a functional relation *)
+  Lemma has_method_fun: ∀ A name mdef0 mdef1 orig0 orig1,
+    has_method name A orig0 mdef0 → has_method name A orig1 mdef1 →
+    orig0 = orig1 ∧ mdef0 = mdef1.
+  Proof.
+    move => A name mdef0 mdef1 orig0 orig1 h; move: mdef1.
+    induction h as [ current cdef mdef hΔ hm 
+      | current parent orig inst cdef mdef hΔ hm hs hp hi ] => mdef1 h1.
+    - inv h1; by simplify_eq.
+    - inv h1.
+      + by simplify_eq.
+      + simplify_eq.
+        apply hi in H2 as []; by subst.
+  Qed.
 
-    Fixpoint expr_eval (le : local_env) (e: expr) : option value :=
-      match e with
-      | IntE z => Some (IntV z)
-      | BoolE b => Some (BoolV b)
-      | NullE => Some NullV
-      | OpE op e1 e2 =>
-          match expr_eval le e1, expr_eval le e2 with 
-          | Some (IntV z1), Some (IntV z2) => Some (primop_eval op z1 z2)
-          | _, _ => None
-          end
-      | VarE v => le !! v
-      end
-    .
+  (* any redeclared method must correctly override its parent methods *)
+  Definition wf_method_override (prog: stringmap classDef) :=
+    ∀ A B adef bdef m σ mA mB,
+    prog !! A = Some adef →
+    prog !! B = Some bdef →
+    inherits_using A B σ →
+    adef.(classmethods) !! m = Some mA →
+    bdef.(classmethods) !! m = Some mB →
+    mdef_incl mA (subst_mdef σ mB).
 
-    (* concrete heaps *)
-    Definition heap : Type := gmap loc (tag * stringmap value).
+  (* Helper lemma that gives all the relevant info from a has_method
+   * statement:
+   * - the class where it was originall defined
+   * - the substitutions needed to interpret it in A, or in its original
+   *   location.
+   *)
+  Lemma has_method_from_def A m orig mdef:
+    map_Forall (λ _cname, wf_cdef_parent Δ) Δ →
+    map_Forall (λ _cname, cdef_methods_bounded) Δ →
+    has_method m A orig mdef →
+    ∃ cdef mdef_orig,
+      Δ !! orig = Some cdef ∧
+      cdef.(classmethods) !! m = Some mdef_orig ∧
+      has_method m orig orig mdef_orig ∧
+      ∃ σ, inherits_using A orig σ ∧ mdef = subst_mdef σ mdef_orig.
+  Proof.
+    move => /map_Forall_lookup hp /map_Forall_lookup hmb.
+    induction 1 as [ A adef mdef hΔ hm | A parent orig σ cdef mdef hΔ hm hs h hi ].
+    - exists adef, mdef; repeat split => //; first by econstructor.
+      exists (gen_targs adef.(generics)); split; first by constructor.
+      rewrite subst_mdef_gen_targs //.
+      apply hmb in hΔ.
+      by apply hΔ in hm.
+    - destruct hi as (odef & omdef & ho & hom & hdef & [σo [hin ->]]).
+      exists odef, omdef; repeat split => //.
+      exists (subst_ty σ <$> σo); split.
+      { econstructor; last done.
+        by econstructor.
+      }
+      rewrite subst_mdef_mdef //.
+      assert (ho' := ho).
+      apply hmb in ho.
+      apply ho in hom.
+      apply inherits_using_wf in hin as (? & ? & ? & ? & ? & hlen & _) => //.
+      simplify_eq.
+      by rewrite hlen.
+  Qed.
 
-    Definition map_args {A B: Type} (f: A → option  B) (m: stringmap A) :
-      option (stringmap B) :=
-      guard (map_Forall (λ _ x, is_Some (f x)) m); Some (omap f m)
-    .
+  (* Helper lemma: If A inherits a method m from class orig, and
+   * A <: B <: orig, then B must also inherits method m from orig.
+   *)
+  Lemma has_method_below_orig A m orig mdef:
+    wf_no_cycle Δ →
+    map_Forall (λ _cname, wf_cdef_parent Δ) Δ →
+    map_Forall (λ _cname, cdef_methods_bounded) Δ →
+    has_method m A orig mdef →
+    ∀ B σ σ', inherits_using A B σ → inherits_using B orig σ' →
+    ∃ odef mdefo mdefB,
+    Δ !! orig = Some odef ∧
+    odef.(classmethods) !! m = Some mdefo ∧
+    has_method m B orig mdefB ∧
+    mdefB = subst_mdef σ' mdefo.
+  Proof.
+    move => hc hp hb.
+    induction 1 as [ A cdef mdef hΔ hm | A parent orig σ cdef mdef hΔ hm hs h hi ] =>
+          B σA σB hAB hBO.
+    - destruct (hc _ _ _ _ hAB hBO) as [-> ->].
+      apply inherits_using_refl in hAB as [ ? [? ->]] => // ; simplify_eq.
+      exists cdef, mdef, mdef; repeat split => //.
+      + by econstructor.
+      + rewrite subst_mdef_gen_targs //.
+        rewrite map_Forall_lookup in hb.
+        apply hb in hΔ.
+        by apply hΔ in hm.
+    - inv hAB.
+      + simplify_eq.
+        destruct (has_method_from_def _ _ _ _ hp hb h) as (odef & modef & ? & hmo & _ & [σo [hin ->]]).
+        exists odef, modef, (subst_mdef σ (subst_mdef σo modef)); repeat split => //.
+        * by econstructor.
+        * assert (hσ: subst_ty σ <$> σo = σB).
+          { eapply inherits_using_fun => //.
+            eapply InheritsTrans; last done.
+            by econstructor.
+          }
+          rewrite subst_mdef_mdef; first by rewrite hσ.
+          apply inherits_using_wf in hBO as (? & ? & ? & ? & hF & hL & _) => //; simplify_eq.
+          apply hb in H1.
+          apply H1 in hmo.
+          rewrite map_Forall_lookup in hp.
+          rewrite map_length in hL.
+          by rewrite hL.
+      + inv H; simplify_eq; clear hi.
+        destruct (has_method_from_def _ _ _ _ hp hb h) as (odef & modef & ? & hmo & _ & [σo [hin ->]]).
+        exists odef, modef, (subst_mdef σo modef); repeat split => //.
+        replace σB with σo; first done.
+        by eapply inherits_using_fun.
+      + inv H; simplify_eq.
+        destruct (hi _ _ _ H0 hBO) as (odef & mdefo & mdefB & ? & ? & ? & ->).
+        by exists odef, mdefo, (subst_mdef σB mdefo).
+  Qed.
 
-    Lemma dom_map_args: ∀ A B (f: A → option B)
-      (m: stringmap A) (n: stringmap B),
-      map_args f m = Some n → 
-      dom stringset n = dom _ m.
-    Proof.
-      rewrite /map_args => A B f m n h.
-      case_option_guard; last done.
-      injection h; intros <-; clear h.
-      rewrite -> map_Forall_lookup in H.
-      apply set_eq => x; split; move/elem_of_dom => hx; apply elem_of_dom.
-      - rewrite lookup_omap in hx.
-        destruct hx as [v hv]; by apply bind_Some in hv as [a [-> ha]].
-      - destruct hx as [v hv].
-        rewrite lookup_omap hv.
-        by apply H in hv.
-    Qed.
+  (* Key lemma for adequacy of method call:
+   * if A <: B and they both have a method m (from resp. origA, origB), then
+   * the origins must be ordered in the same way, meaning origA <: origB.
+   * This implies some relations on all the inheritance substitution.
+   *)
+  Lemma has_method_ordered A B σ m origA mdefA origB mdefB:
+    wf_no_cycle Δ →
+    wf_method_override Δ →
+    map_Forall (λ _cname, wf_cdef_parent Δ) Δ →
+    map_Forall (λ _cname, cdef_methods_bounded) Δ →
+    inherits_using A B σ →
+    has_method m A origA mdefA →
+    has_method m B origB mdefB →
+    ∃ σin σA σB oA oB mA mB,
+      subst_ty σ <$> σB = subst_ty σA <$> σin ∧
+      Δ !! origA = Some oA ∧
+      Δ !! origB = Some oB ∧
+      oA.(classmethods) !! m = Some mA ∧
+      oB.(classmethods) !! m = Some mB ∧
+      inherits_using origA origB σin ∧
+      inherits_using A origA σA ∧
+      inherits_using B origB σB ∧
+      has_method m origA origA mA ∧ (* Not sure these are useful *)
+      has_method m origB origB mB ∧
+      mdefA = subst_mdef σA mA ∧
+      mdefB = subst_mdef σB mB ∧
+      mdef_incl mA (subst_mdef σin mB) ∧
+      mdef_incl mdefA (subst_mdef σ mdefB).
+  Proof.
+    move => hc ho hp hm hin hA hB.
+    assert (hhA := hA).
+    assert (hhB := hB).
+    apply has_method_from_def in hA => //.
+    apply has_method_from_def in hB => //.
+    destruct hA as (oadef & oaorig & hoA & hmA & hmoA & [σA [hiA ->]]).
+    destruct hB as (obdef & oborig & hoB & hmB & hmoB & [σB [hiB ->]]).
+    destruct (inherits_using_chain _ _ _ hp hin _ _ hiA) as [σ'' [ [<- h] | [<- h]]].
+    - destruct (has_method_below_orig _ _ _ _ hc hp hm hhA _ _ _ hin h) as
+        (? & ? & mbdef & ? & ? & hbm & ->); simplify_eq.
+      destruct (has_method_fun _ _ _ _ _ _ hhB hbm) as [-> ->].
+      simplify_eq.
+      exists (gen_targs oadef.(generics)),
+             (subst_ty σ <$> σ''),
+             σ'',
+             oadef, oadef,
+             oaorig, oaorig.
+      split.
+      { rewrite subst_ty_gen_targs //.
+        apply inherits_using_wf in hiA => //.
+        repeat destruct hiA as [? hiA]; by simplify_eq.
+      }
+      do 4 (split => //).
+      split; first by econstructor.
+      do 6 (split => //).
+      split.
+      + repeat split.
+        * by rewrite /subst_mdef /= dom_fmap_L.
+        * move => k X Y hX.
+          rewrite /subst_mdef /= lookup_fmap hX /= subst_ty_id.
+          { by case => ->. }
+          apply hm in hoA.
+          apply hoA in hmA.
+          by apply hmA in hX.
+        * rewrite /subst_mdef /= subst_ty_id //.
+          apply hm in hoA.
+          by apply hoA in hmA as [].
+      + rewrite subst_mdef_mdef; first by apply mdef_incl_reflexive.
+        assert (hoA' := hoA).
+        apply hm in hoA'.
+        apply hoA' in hmA.
+        apply inherits_using_wf in h => //.
+        repeat destruct h as [? h]; simplify_eq.
+        by rewrite H2.
+    - exists (subst_ty σ'' <$> σB), σA, σB, oadef, obdef, oaorig, oborig.
+      split.
+      { rewrite map_subst_ty_subst //.
+        apply inherits_using_wf in hiB => //.
+        repeat destruct hiB as [? hiB].
+        apply inherits_using_wf in h => //.
+        repeat destruct h as [? h].
+        simplify_eq.
+        by rewrite H6.
+      }
+      assert (hh: inherits_using origA origB (subst_ty σ'' <$> σB))
+        by (by eapply inherits_using_trans).
+      assert (hincl : mdef_incl oaorig (subst_mdef (subst_ty σ'' <$> σB) oborig))
+        by (by eapply (ho origA origB) in hh).
+      do 12 (split => //).
+      rewrite -subst_mdef_mdef; last first.
+      { assert (hoB' := hoB).
+        apply hm in hoB'.
+        apply hoB' in hmB.
+        apply inherits_using_wf in hiB => //.
+        repeat destruct hiB as [? hiB].
+        simplify_eq.
+        apply bounded_subst_mdef with (generics obdef) => //.
+        apply inherits_using_wf in h => //.
+        repeat destruct h as [? h].
+        simplify_eq.
+        rewrite Forall_forall => ty hty.
+        rewrite H5.
+        rewrite Forall_forall in H1.
+        by apply H1 in hty.
+      }
+      apply mdef_incl_subst => //.
+      { apply inherits_using_wf in hiA => //.
+        by repeat destruct hiA as [? hiA].
+      }
+      rewrite subst_mdef_mdef //.
+      { assert (hoB' := hoB).
+        apply hm in hoB'.
+        apply hoB' in hmB.
+        apply inherits_using_wf in hiB => //.
+        repeat destruct hiB as [? hiB].
+        simplify_eq.
+        by rewrite H2.
+      }
+  Qed.
 
-    Lemma map_args_lookup: ∀ A B (f: A → option B) (m: stringmap A) n,
-      map_args f m = Some n →
-      ∀ k, n !! k = (m !! k) ≫= f.
-    Proof.
-      rewrite /map_args => A B f m n h k.
-      case_option_guard; last done.
-      injection h; intros <-; clear h.
-      rewrite -> map_Forall_lookup in H.
-      by rewrite lookup_omap.
-    Qed.
+  (* Typing Judgements *)
+  Definition is_bool_op op : bool :=
+    match op with
+    | LeqO | GeqO | EqO => true
+    | PlusO | MinusO | TimesO | DivO => false
+    end
+  .
 
-    Lemma map_args_empty: ∀ A B (f: A → option B),
-      map_args f ∅ = Some ∅.
-    Proof.
-      rewrite /map_args => A B f /=.
-      case_option_guard; first by rewrite omap_empty.
-      elim: H.
-      apply map_Forall_lookup => i x h; discriminate h.
-    Qed.
+  Inductive expr_has_ty (lty : local_tys) :
+    expr → lang_ty → Prop :=
+    | IntTy : ∀ z, expr_has_ty lty (IntE z) IntT
+    | BoolTy: ∀ b, expr_has_ty lty (BoolE b) BoolT
+    | NullTy: expr_has_ty lty NullE NullT
+    | OpIntTy: ∀ op e1 e2,
+        is_bool_op op = false →
+        expr_has_ty lty e1 IntT →
+        expr_has_ty lty e2 IntT →
+        expr_has_ty lty (OpE op e1 e2) IntT
+    | OpBoolTy: ∀ op e1 e2,
+        is_bool_op op = true →
+        expr_has_ty lty e1 IntT →
+        expr_has_ty lty e2 IntT →
+        expr_has_ty lty (OpE op e1 e2) BoolT
+    | GenTy: ∀ v ty,
+        lty !! v = Some ty →
+        expr_has_ty lty (VarE v) ty
+    | ESubTy: ∀ e s t,
+        expr_has_ty lty e s →
+        wf_ty t →
+        s <: t →
+        expr_has_ty lty e t
+  .
 
-    Lemma map_args_update: ∀ A B (f: A → option B) k a m n,
-      map_args f m = Some n →
-      map_args f (<[ k := a]> m) =
-      match f a with
-      | Some b => Some (<[ k := b]> n)
-      | None => None
-      end.
-    Proof.
-      rewrite /map_args => A B f k a m n h /=.
-      case_option_guard; last done.
-      injection h; intros <-; clear h.
-      case_option_guard.
-      - rewrite map_Forall_lookup in H0.
-        specialize H0 with k a.
-        rewrite lookup_insert in H0.
-        destruct H0 as [ b hb ]; first by done.
-        rewrite hb.
-        f_equal.
-        by apply omap_insert_Some.
-      - destruct (f a) as [b | ] eqn:hb; last done.
-        elim: H0 => i x h.
-        rewrite lookup_insert_Some in h.
-        destruct h as [[<- <-] | [hne hin]]; first by rewrite hb.
-        rewrite map_Forall_lookup in H.
-        now apply H in hin.
-    Qed.
+  Lemma expr_has_ty_subst σ lty e ty:
+    map_Forall (λ _ : string, wf_cdef_parent Δ) Δ →
+    Forall wf_ty σ →
+    expr_has_ty lty e ty →
+    expr_has_ty (subst_ty σ <$> lty) e (subst_ty σ ty).
+  Proof.
+    move => hp hwf.
+    induction 1 as [ z | b | | op e1 e2 hop h1 hi1 h2 hi2 |
+      op e1 e2 hop h1 hi1 h2 hi2 | v ty h | e s t h hi hsub ] => //=; try (by constructor).
+    - constructor.
+      by rewrite lookup_fmap h.
+    - econstructor; first by apply hi.
+      + by apply wf_ty_subst.
+      + by apply subtype_subst.
+  Qed.
 
-    Definition tag_match (st : local_env * heap) (v: string) (t: tag) :=
-      ∃ l, st.1 !! v = Some (LocV l) ∧
-      ∃ t' (fields: stringmap value), st.2 !! l = Some (t', fields) ∧
-      inherits t' t
-    .
+  Lemma expr_has_ty_wf lty e ty:
+    map_Forall (λ _, wf_ty) lty →
+    expr_has_ty lty e ty →
+    wf_ty ty.
+  Proof.
+    move => hwf.
+    induction 1 as [ z | b | | op e1 e2 hop h1 hi1 h2 hi2 |
+      op e1 e2 hop h1 hi1 h2 hi2 | v ty h | e s t h hi hsub ] => //=; try (by constructor).
+    rewrite map_Forall_lookup in hwf.
+    by apply hwf in h.
+  Qed.
 
-    Inductive cmd_eval:
-      (local_env * heap) → cmd →
-      (local_env * heap) → nat → Prop :=
-      | SkipEv : ∀ st, cmd_eval st SkipC st 0
-      | LetEv: ∀ le h v e val,
-          expr_eval le e = Some val →
-          cmd_eval (le, h) (LetC v e) (<[v := val]> le, h) 0
-      | NewEv: ∀ le h lhs new t args vargs,
-          h !! new = None →
-          map_args (expr_eval le) args = Some vargs →
-          cmd_eval (le, h) (NewC lhs t args) (<[lhs := LocV new]>le, <[new := (t, vargs)]>h) 1
-      | GetEv: ∀ le h lhs recv name l t vs v,
-          expr_eval le recv = Some (LocV l) →
-          h !! l = Some (t, vs) →
-          vs !! name = Some v →
-          cmd_eval (le, h) (GetC lhs recv name) (<[lhs := v]>le, h) 1
-      | SetEv: ∀ le h recv fld rhs l v t vs vs',
-          expr_eval le recv = Some (LocV l) →
-          expr_eval le rhs = Some v →
-          h !! l = Some (t, vs) →
-          vs' = <[ fld := v ]>vs →
-          cmd_eval (le, h) (SetC recv fld rhs) (le, <[l := (t, vs')]> h) 0
-      | SeqEv: ∀ st1 st2 st3 fstc sndc n1 n2,
-          cmd_eval st1 fstc st2 n1 →
-          cmd_eval st2 sndc st3 n2 →
-          cmd_eval st1 (SeqC fstc sndc) st3 (n1 + n2)
-      | IfTrueEv: ∀ st1 st2 cond thn els n,
-          expr_eval st1.1 cond = Some (BoolV true) →
-          cmd_eval st1 thn st2 n →
-          cmd_eval st1 (IfC cond thn els) st2 n
-      | IfFalseEv: ∀ st1 st2 cond thn els n,
-          expr_eval st1.1 cond = Some (BoolV false) →
-          cmd_eval st1 els st2 n →
-          cmd_eval st1 (IfC cond thn els) st2 n
-      | CallEv: ∀ le h h' lhs recv l t vs name args vargs mdef
-          run_env run_env' ret n,
-          expr_eval le recv = Some (LocV l) →
-          map_args (expr_eval le) args = Some vargs →
-          h !! l = Some (t, vs) →
-          has_method name mdef t →
-          <["$this" := LocV l]>vargs = run_env →
-          cmd_eval (run_env, h) mdef.(methodbody) (run_env', h') n →
-          expr_eval run_env' mdef.(methodret) = Some ret →
-          cmd_eval (le, h) (CallC lhs recv name args) (<[lhs := ret]>le, h') (S n)
-      | CondTag1Ev n st1 st2 v t cmd :
-          (* tag in heap must <: requested tag to move forward *)
-          tag_match st1 v t →
-          cmd_eval st1 cmd st2 n →
-          cmd_eval st1 (CondTagC v t cmd) st2 n
-      | CondTag2Ev n st v t cmd :
-          ¬tag_match st v t →
-          cmd_eval st (CondTagC v t cmd) st n
+  (* continuation-based typing for commands *)
+  Inductive cmd_has_ty :
+    local_tys → cmd → local_tys → Prop :=
+    | SkipTy: ∀ lty, cmd_has_ty lty SkipC lty
+    | SeqTy: ∀ lty1 lty2 lty3 fstc sndc,
+        cmd_has_ty lty1 fstc lty2 →
+        cmd_has_ty lty2 sndc lty3 →
+        cmd_has_ty lty1 (SeqC fstc sndc) lty3
+    | LetTy: ∀ lty lhs e ty,
+        expr_has_ty lty e ty →
+        cmd_has_ty lty (LetC lhs e) (<[lhs := ty]>lty)
+    | IfTy: ∀ lty1 lty2 cond thn els,
+        expr_has_ty lty1 cond BoolT →
+        cmd_has_ty lty1 thn lty2 →
+        cmd_has_ty lty1 els lty2 →
+        cmd_has_ty lty1 (IfC cond thn els) lty2
+    | GetTy: ∀ lty lhs recv t σ name fty,
+        expr_has_ty lty recv (ClassT t σ) →
+        has_field name t fty →
+        cmd_has_ty lty (GetC lhs recv name) (<[lhs := subst_ty σ fty]>lty)
+    | SetTy: ∀ lty recv fld rhs fty t σ,
+        expr_has_ty lty recv (ClassT t σ) →
+        has_field fld t fty →
+        expr_has_ty lty rhs (subst_ty σ fty) →
+        cmd_has_ty lty (SetC recv fld rhs) lty
+    | NewTy: ∀ lty lhs t targs args fields (*cdef*),
+        wf_ty (ClassT t targs) →
+        has_fields t fields →
+        dom (gset string) fields = dom _ args →
+        (∀ f fty arg,
+        fields !! f = Some fty →
+        args !! f = Some arg →
+        expr_has_ty lty arg (subst_ty targs fty)) →
+        cmd_has_ty lty (NewC lhs t args) (<[lhs := ClassT t targs]>lty)
+    | CallTy: ∀ lty lhs recv t targs name orig mdef args,
+        expr_has_ty lty recv (ClassT t targs) →
+        has_method name t orig mdef →
+        dom (gset string) mdef.(methodargs) = dom _ args →
+        (∀ x ty arg,
+        mdef.(methodargs) !! x = Some ty →
+        args !! x = Some arg →
+        expr_has_ty lty arg (subst_ty targs ty)) →
+        cmd_has_ty lty (CallC lhs recv name args) (<[lhs := subst_ty targs mdef.(methodrettype)]>lty)
+    | SubTy: ∀ lty c rty rty',
+        rty' <:< rty →
+        cmd_has_ty lty c rty' →
+        cmd_has_ty lty c rty
+    | CondTagTy lty rty v tv t cmd :
+        lty !! v = Some tv →
+        lty <:< rty →
+        cmd_has_ty (<[v:=InterT tv (ExT t)]> lty) cmd rty →
+        cmd_has_ty lty (CondTagC v t cmd) rty
+  .
+
+  Lemma cmd_has_ty_wf lty cmd lty' :
+    map_Forall (λ _ : string, wf_cdef_parent Δ) Δ →
+    map_Forall (λ _ : string, wf_cdef_fields_wf) Δ →
+    map_Forall (λ _ : string, wf_cdef_methods_wf) Δ →
+    map_Forall (λ _, wf_ty) lty →
+    cmd_has_ty lty cmd lty' →
+    map_Forall (λ _, wf_ty) lty'.
+  Proof.
+    move => hp hfields hmethods hwf.
+    induction 1 as [ lty | ????? h1 hi1 h2 hi2 | ???? he |
+      ????? he h1 hi1 h2 hi2 | ??????? he hf |
+      ??????? he hf hr | ?????? ht hf hdom hargs |
+      ????????? he hm hdom hargs |
+      ???? hsub h hi | ?????? hin hr h hi ] => //=; try (by eauto).
+    - apply map_Forall_insert_2 => //.
+      by apply expr_has_ty_wf in he.
+    - apply map_Forall_insert_2 => //.
+      apply wf_ty_subst.
+      + apply expr_has_ty_wf in he => //.
+        by apply wf_ty_class_inv in he.
+      + by apply has_field_wf in hf.
+    - by apply map_Forall_insert_2.
+    - apply map_Forall_insert_2 => //.
+      apply has_method_wf in hm => //.
+      destruct hm as [hargs' hret'].
+      apply wf_ty_subst => //.
+      apply expr_has_ty_wf in he => //.
+      by apply wf_ty_class_inv in he.
+    - apply hi in hwf; clear hi h.
+      rewrite map_Forall_lookup => k ty hty.
+      apply hsub in hty.
+      destruct hty as [ty' [ hty' hsub']].
+      rewrite map_Forall_lookup in hwf; apply hwf in hty'.
+      by eapply subtype_wf.
+    - apply hi; clear hi.
+      rewrite map_Forall_lookup => k ty.
+      rewrite lookup_insert_Some.
+      case => [[heq <-] | [hne hk]].
+      { constructor; last by constructor.
+        by apply hwf in hin.
+      }
+      by apply hwf in hk.
+  Qed.
+
+  Lemma cmd_has_ty_subst σ lty cmd lty':
+    map_Forall (λ _ : string, wf_cdef_parent Δ) Δ →
+    map_Forall (λ _ : string, wf_cdef_fields_wf) Δ →
+    map_Forall (λ _ : string, wf_cdef_methods_wf) Δ →
+    map_Forall (λ _ : string, wf_cdef_fields_bounded) Δ →
+    map_Forall (λ _ : string, cdef_methods_bounded) Δ →
+    map_Forall (λ _, wf_ty) lty →
+    Forall wf_ty σ →
+    cmd_has_ty lty cmd lty' →
+    cmd_has_ty (subst_ty σ <$> lty) cmd (subst_ty σ <$> lty').
+  Proof.
+    move => hp hfields hmethods hfb hmb hwf0 hwf1.
+    induction 1 as [ lty | ????? h1 hi1 h2 hi2 | ???? he |
+      ????? he h1 hi1 h2 hi2 | ??????? he hf |
+      ??????? he hf hr | ?????? hwf hf hdom hargs |
+      ????????? he hm hdom hargs |
+      ???? hsub h hi | ?????? hin hr h hi ] => //=.
+    - by constructor.
+    - econstructor.
+      + by eapply hi1.
+      + eapply hi2.
+        by apply cmd_has_ty_wf in h1.
+    - rewrite fmap_insert.
+      eapply LetTy.
+      by eapply expr_has_ty_subst.
+    - eapply IfTy => //.
+      + change BoolT with (subst_ty σ BoolT).
+        by eapply expr_has_ty_subst.
+      + by apply hi1.
+      + apply hi2.
+        by apply cmd_has_ty_wf in h1.
+    - rewrite fmap_insert subst_ty_subst; last first.
+      { apply has_field_bounded in hf => //.
+        destruct hf as (hdef & ht & hfty).
+        apply expr_has_ty_wf in he => //.
+        inv he; simplify_eq.
+        by rewrite H2.
+      }
+      eapply GetTy; last done.
+      change (ClassT t (subst_ty σ <$> σ0)) with (subst_ty σ (ClassT t σ0)).
+      by eapply expr_has_ty_subst.
+    - apply SetTy with (fty := fty) (t := t) (σ := subst_ty σ <$> σ0) => //; last first.
+      + rewrite -subst_ty_subst; first by eapply expr_has_ty_subst.
+        apply has_field_bounded in hf => //.
+        destruct hf as (hdef & ht & hfty).
+        apply expr_has_ty_wf in he => //.
+        inv he; simplify_eq.
+        by rewrite H2.
+      + change (ClassT t (subst_ty σ <$> σ0)) with (subst_ty σ (ClassT t σ0)).
+        by eapply expr_has_ty_subst.
+    - rewrite fmap_insert /=.
+      eapply NewTy => //.
+      { inv hwf.
+        econstructor => //; first by rewrite map_length.
+        move => k ty.
+        rewrite list_lookup_fmap.
+        destruct (targs !! k) as [ ty' | ] eqn:hty' => //=.
+        case => <-.
+        apply wf_ty_subst => //.
+        by apply H3 in hty'.
+      }
+      move => f fty arg hfty ha.
+      rewrite -subst_ty_subst.
+      + eapply expr_has_ty_subst => //.
+        by eapply hargs.
+      + apply hf in hfty.
+        apply has_field_bounded in hfty => //.
+        destruct hfty as (hdef & ht & hfty).
+        inv hwf; simplify_eq.
+        by rewrite H2.
+    - rewrite fmap_insert /=.
+      rewrite subst_ty_subst; last first.
+      { apply has_method_from_def in hm => //.
+        destruct hm as (odef & mo & ho & hmo & _ & [σo [hin ->]]).
+        rewrite /subst_mdef /=.
+        rewrite map_Forall_lookup in hmb.
+        apply inherits_using_wf in hin => //.
+        destruct hin as (tdef & ? & ht & ho' & hfo & hlo & htyo); simplify_eq.
+        assert (ho' := ho).
+        apply hmb in ho.
+        apply ho in hmo.
+        destruct hmo as [_ hret].
+        apply bounded_subst with (n := generics odef) => //.
+        apply expr_has_ty_wf in he => //.
+        inv he; simplify_eq.
+        by rewrite H2.
+      }
+      eapply CallTy => //.
+      + change (ClassT t (subst_ty σ <$> targs)) with (subst_ty σ (ClassT t targs)).
+        by eapply expr_has_ty_subst.
+      + move => x ty arg hty ha.
+        rewrite -subst_ty_subst.
+        { eapply expr_has_ty_subst => //.
+          by eapply hargs.
+        }
+        apply has_method_from_def in hm => //.
+        destruct hm as (odef & mo & ho & hmo & _ & [σo [hin ->]]).
+        rewrite map_Forall_lookup in hmb.
+        apply inherits_using_wf in hin => //.
+        destruct hin as (tdef & ? & ht & ho' & hfo & hlo & htyo); simplify_eq.
+        assert (ho' := ho).
+        apply hmb in ho.
+        apply ho in hmo.
+        destruct hmo as [hargs' _].
+        rewrite map_Forall_lookup in hargs'.
+        rewrite /subst_mdef /= in hty.
+        rewrite lookup_fmap_Some in hty.
+        destruct hty as [ty' [ <- hty]].
+        apply hargs' in hty.
+        apply bounded_subst with (n := generics odef) => //.
+        apply expr_has_ty_wf in he => //.
+        inv he; simplify_eq.
+        by rewrite H2.
+    - econstructor; first by apply lty_sub_subst.
+      by apply hi.
+    - eapply CondTagTy.
+      + by rewrite lookup_fmap hin /=.
+      + by apply lty_sub_subst.
+      + rewrite fmap_insert /= in hi.
+        apply hi.
+        apply map_Forall_insert_2 => //.
+        constructor; last by constructor.
+        rewrite map_Forall_lookup in hwf0.
+        by apply hwf0 in hin.
+  Qed.
+
+  (* Consider a class C<T0, ..., Tn>,
+   * method bodies must be well-formed under a generic substitution mapping
+   * Ti -> Ti.
+   *)
+  Definition wf_mdef_ty this σ mdef :=
+    ∃ rty,
+    cmd_has_ty (<["$this" := this]>(subst_ty σ <$> mdef.(methodargs))) mdef.(methodbody) rty ∧
+    expr_has_ty rty mdef.(methodret) (subst_ty σ mdef.(methodrettype))
+  .
+
+  Definition cdef_wf_mdef_ty cname cdef :=
+    let σ := gen_targs cdef.(generics) in
+    map_Forall (λ _mname mdef, wf_mdef_ty (ClassT cname σ) σ mdef) cdef.(classmethods)
+  .
+
+  (* Collection of all program invariant (at the source level):
+   * - no cycle (we have a forest)
+   * - every type is well-formed/bounded
+   * - every substitution's domain/codomain is valid
+   *)
+  Record wf_cdefs (prog: stringmap classDef) := {
+    wf_extends_wf : wf_no_cycle prog;
+    wf_parent : map_Forall (λ _cname, wf_cdef_parent prog) prog;
+    wf_override : wf_method_override Δ;
+    wf_fields : map_Forall (λ _cname, wf_cdef_fields) prog;
+    wf_fields_bounded : map_Forall (λ _cname, wf_cdef_fields_bounded) prog;
+    wf_fields_wf  : map_Forall (λ _cname, wf_cdef_fields_wf) prog;
+    wf_methods_bounded : map_Forall (λ _cname, cdef_methods_bounded) prog;
+    wf_methods_wf : map_Forall (λ _cname, wf_cdef_methods_wf) prog;
+    wf_mdefs : map_Forall cdef_wf_mdef_ty prog;
+  }
+  .
+
+  Lemma expr_has_ty_subl lty e ty:  
+    map_Forall (λ _, wf_ty) lty →
+    expr_has_ty lty e ty →
+    ∀ lty', lty' <:< lty →
+    expr_has_ty lty' e ty.
+  Proof.
+    move => hwf.
+    induction 1 as [ z | b | | op e1 e2 hop h1 hi1 h2 hi2 |
+      op e1 e2 hop h1 hi1 h2 hi2 | v ty h | e s t h hi hsub ] => lty' hlty//=; try (by constructor).
+    - constructor; by eauto.
+    - constructor; by eauto.
+    - assert (hh : wf_ty ty) by (by apply hwf in h).
+      apply hlty in h.
+      destruct h as [ty' [ h hsub]].
+      eapply ESubTy => //.
+      by constructor.
+    - apply hi in hlty.
+      by econstructor.
+  Qed.
+
+  Lemma cmd_has_ty_subl lty cmd rty :
+    map_Forall (λ _ : string, wf_cdef_parent Δ) Δ →
+    map_Forall (λ _ : string, wf_ty) lty →
+    cmd_has_ty lty cmd rty →
+    ∀ lty', lty' <:< lty →
+    cmd_has_ty lty' cmd rty.
+  Proof.
+    move => hp hwf.
+    induction 1 as [ lty | ????? h1 hi1 h2 hi2 | ???? he |
+      ????? he h1 hi1 h2 hi2 | ??????? he hf |
+      ??????? he hf hr | ?????? ht hf hdom hargs |
+      ????????? he hm hdom hargs |
+      ???? hsub h hi | ?????? hin hr h hi ] => //= lty' hlty'.
+    - apply SubTy with lty' => //.
+      by constructor.
+    - econstructor; by eauto.
+    - eapply SubTy; first by apply lty_sub_insert_1.
+      constructor.
+      by apply expr_has_ty_subl with lty.
+    - constructor; try (by eauto).
+      by apply expr_has_ty_subl with lty1.
+    - eapply SubTy; first by apply lty_sub_insert_1.
+      econstructor; last done.
+      by apply expr_has_ty_subl with lty.
+    - apply SubTy with lty' => //.
+      econstructor; [| done|]; by eapply expr_has_ty_subl.
+    - eapply SubTy; first by apply lty_sub_insert_1.
+      econstructor => //.
+      move => f fty arg hfty ha.
+      eapply expr_has_ty_subl => //.
+      by eapply hargs.
+    - eapply SubTy; first by apply lty_sub_insert_1.
+      econstructor => //.
+      + by eapply expr_has_ty_subl.
+      + move => f fty arg hfty ha.
+        eapply expr_has_ty_subl => //.
+        by eapply hargs.
+    - econstructor; by eauto.
+    - destruct (hlty' _ _ hin) as [ty' [? ?]].
+      eapply CondTagTy.
+      + done.
+      + by eapply lty_sub_transitive.
+      + eapply hi.
+        * rewrite map_Forall_lookup => x tx.
+          rewrite lookup_insert_Some.
+          case => [[? <-] | [? hx]].
+          { constructor; last by constructor.
+            by apply hwf in hin.
+          }
+          by apply hwf in hx.
+        * eapply lty_sub_transitive; first by apply lty_sub_insert_1.
+          apply lty_sub_insert_2.
+          by eauto.
+  Qed.
+
+  Lemma wf_mdef_ty_inherits t0 t σ m mdef orig def def0:
+    map_Forall (λ _ : string, wf_cdef_parent Δ) Δ →
+    map_Forall (λ _ : string, wf_cdef_fields_wf) Δ →
+    map_Forall (λ _ : string, wf_cdef_methods_wf) Δ →
+    map_Forall (λ _ : string, wf_cdef_fields_bounded) Δ →
+    map_Forall (λ _ : string, cdef_methods_bounded) Δ →
+    Δ !! t = Some def →
+    Δ !! t0 = Some def0 →
+    has_method m t orig mdef →
+    wf_mdef_ty (ClassT t (gen_targs def.(generics))) (gen_targs def.(generics)) mdef →
+    inherits_using t0 t σ →
+    wf_mdef_ty (ClassT t0 (gen_targs def0.(generics))) σ mdef.
+  Proof.
+    move => hp hfwf hmwf hfb hmb hΔt hΔt0 hm [rty [hbody hret]] hin.
+    assert (h: Forall (bounded (generics def0)) σ
+            ∧ length σ = generics def ∧ Forall wf_ty σ).
+    { apply inherits_using_wf in hin => //.
+      destruct hin as (? & ? & ? & ? &? & ? & ?).
+      by simplify_eq.
+    }
+    destruct h as (hF & hL & hσ).
+    apply has_method_from_def in hm => //.
+    destruct hm as (def' & mdef_orig & ho & hmdef_orig & _ & σm & hσm & hmdef).
+    apply inherits_using_wf in hσm => //.
+    destruct hσm as (def'' & odef'' & ? & ? & ? & ? & ? );
+    assert (ho' := ho).
+    assert (hmdef_orig' := hmdef_orig).
+    apply hmwf in ho'.
+    apply ho' in hmdef_orig' as [hargs _].
+    exists (subst_ty σ <$> rty); split.
+    - apply cmd_has_ty_subl with (<["$this":=ClassT t σ]>(subst_ty σ <$> methodargs mdef)) => //.
+      + rewrite map_Forall_lookup => x tx.
+        rewrite lookup_insert_Some.
+        simplify_eq.
+        case => [[? <-]|[? ]].
+        * econstructor => //.
+          rewrite Forall_forall in hσ => k ty hk.
+          apply elem_of_list_lookup_2 in hk.
+          by apply hσ.
+        * rewrite lookup_fmap_Some.
+          case => [ty [<- ]].
+          rewrite /subst_mdef /=.
+          rewrite lookup_fmap_Some.
+          case => [tz [<- hz]].
+          apply wf_ty_subst => //.
+          apply wf_ty_subst => //.
+          by apply hargs in hz.
+      + replace (ClassT t σ) with (subst_ty σ (ClassT t (gen_targs def.(generics)))); last first.
+        { by rewrite /= subst_ty_gen_targs. }
+        replace (<["$this":=subst_ty σ (ClassT t (gen_targs (generics def)))]> (subst_ty σ <$> methodargs mdef))
+          with (subst_ty σ <$> (<["$this" := ClassT t (gen_targs (generics def))]> (methodargs mdef))); last first.
+        { by rewrite fmap_insert. }
+        apply cmd_has_ty_subst => //.
+        * rewrite map_Forall_lookup => x tx.
+          rewrite lookup_insert_Some.
+          simplify_eq.
+          case => [[? <-] | [? ]].
+          { econstructor => //; first by rewrite length_gen_targs. 
+            by apply gen_targs_wf.
+          }
+          rewrite /subst_mdef /=.
+          rewrite lookup_fmap_Some.
+          case => [tz [<- hz]].
+          apply wf_ty_subst => //.
+          by apply hargs in hz.
+        * move: hbody.
+          simplify_eq.
+          rewrite fmap_subst_tys_id => //.
+          rewrite map_Forall_lookup /subst_mdef /= => k tk.
+          rewrite lookup_fmap_Some; case => [ty [<- hty]].
+          eapply bounded_subst => //.
+          apply hmb in ho.
+          apply ho in hmdef_orig.
+          by apply hmdef_orig in hty.
+      + move => x tx.
+        rewrite lookup_insert_Some.
+        case => [[<- <-]|[?]].
+        * rewrite lookup_insert.
+          eexists; split => //.
+          replace σ with (subst_ty (gen_targs def0.(generics)) <$> σ); last first.
+          { by rewrite subst_tys_id. }
+          eapply subtype_inherits_using => //.
+          by rewrite length_gen_targs.
+        * rewrite lookup_fmap_Some.
+          case => [ty [<- hx]].
+          rewrite lookup_insert_ne // lookup_fmap hx /=.
+          by eexists.
+    - apply expr_has_ty_subst => //.
+      replace (methodrettype mdef) with (subst_ty (gen_targs (generics def)) (methodrettype mdef)); first done.
+      simplify_eq.
+      rewrite subst_ty_id // /subst_mdef /=.
+      eapply bounded_subst => //.
+      apply hmb in ho.
+      apply ho in hmdef_orig.
+      by apply hmdef_orig.
+  Qed.
+          
+  (* Big step reduction *)
+  Definition primop_eval (op: primop) : Z → Z → value :=
+    match op with
+    | PlusO => fun x y => IntV (x + y)
+    | MinusO => fun x y => IntV (x - y)
+    | TimesO => fun x y => IntV (x * y)
+    | DivO => fun x y => IntV (x / y)
+    | LeqO => fun x y => BoolV (Z.leb x y)
+    | GeqO => fun x y => BoolV (Z.geb x y)
+    | EqO => fun x y => BoolV (Z.eqb x y)
+    end
+  .
+
+  Definition local_env := gmap var value.
+
+  Fixpoint expr_eval (le : local_env) (e: expr) : option value :=
+    match e with
+    | IntE z => Some (IntV z)
+    | BoolE b => Some (BoolV b)
+    | NullE => Some NullV
+    | OpE op e1 e2 =>
+        match expr_eval le e1, expr_eval le e2 with 
+        | Some (IntV z1), Some (IntV z2) => Some (primop_eval op z1 z2)
+        | _, _ => None
+        end
+    | VarE v => le !! v
+    end
+  .
+
+  (* concrete heaps *)
+  Definition heap : Type := gmap loc (tag * stringmap value).
+
+  Definition map_args {A B: Type} (f: A → option  B) (m: stringmap A) :
+    option (stringmap B) :=
+    guard (map_Forall (λ _ x, is_Some (f x)) m); Some (omap f m)
+  .
+
+  Lemma dom_map_args: ∀ A B (f: A → option B)
+    (m: stringmap A) (n: stringmap B),
+    map_args f m = Some n → 
+    dom stringset n = dom _ m.
+  Proof.
+    rewrite /map_args => A B f m n h.
+    case_option_guard; last done.
+    injection h; intros <-; clear h.
+    rewrite -> map_Forall_lookup in H.
+    apply set_eq => x; split; move/elem_of_dom => hx; apply elem_of_dom.
+    - rewrite lookup_omap in hx.
+      destruct hx as [v hv]; by apply bind_Some in hv as [a [-> ha]].
+    - destruct hx as [v hv].
+      rewrite lookup_omap hv.
+      by apply H in hv.
+  Qed.
+
+  Lemma map_args_lookup: ∀ A B (f: A → option B) (m: stringmap A) n,
+    map_args f m = Some n →
+    ∀ k, n !! k = (m !! k) ≫= f.
+  Proof.
+    rewrite /map_args => A B f m n h k.
+    case_option_guard; last done.
+    injection h; intros <-; clear h.
+    rewrite -> map_Forall_lookup in H.
+    by rewrite lookup_omap.
+  Qed.
+
+  Lemma map_args_empty: ∀ A B (f: A → option B),
+    map_args f ∅ = Some ∅.
+  Proof.
+    rewrite /map_args => A B f /=.
+    case_option_guard; first by rewrite omap_empty.
+    elim: H.
+    apply map_Forall_lookup => i x h; discriminate h.
+  Qed.
+
+  Lemma map_args_update: ∀ A B (f: A → option B) k a m n,
+    map_args f m = Some n →
+    map_args f (<[ k := a]> m) =
+    match f a with
+    | Some b => Some (<[ k := b]> n)
+    | None => None
+    end.
+  Proof.
+    rewrite /map_args => A B f k a m n h /=.
+    case_option_guard; last done.
+    injection h; intros <-; clear h.
+    case_option_guard.
+    - rewrite map_Forall_lookup in H0.
+      specialize H0 with k a.
+      rewrite lookup_insert in H0.
+      destruct H0 as [ b hb ]; first by done.
+      rewrite hb.
+      f_equal.
+      by apply omap_insert_Some.
+    - destruct (f a) as [b | ] eqn:hb; last done.
+      elim: H0 => i x h.
+      rewrite lookup_insert_Some in h.
+      destruct h as [[<- <-] | [hne hin]]; first by rewrite hb.
+      rewrite map_Forall_lookup in H.
+      now apply H in hin.
+  Qed.
+
+  Definition tag_match (st : local_env * heap) (v: string) (t: tag) :=
+    ∃ l, st.1 !! v = Some (LocV l) ∧
+    ∃ t' (fields: stringmap value), st.2 !! l = Some (t', fields) ∧
+    inherits t' t
+  .
+
+  Inductive cmd_eval:
+    (local_env * heap) → cmd →
+    (local_env * heap) → nat → Prop :=
+    | SkipEv : ∀ st, cmd_eval st SkipC st 0
+    | LetEv: ∀ le h v e val,
+        expr_eval le e = Some val →
+        cmd_eval (le, h) (LetC v e) (<[v := val]> le, h) 0
+    | NewEv: ∀ le h lhs new t args vargs,
+        (* targs are not stored in the heap: erased generics *)
+        h !! new = None →
+        map_args (expr_eval le) args = Some vargs →
+        cmd_eval (le, h) (NewC lhs t args) (<[lhs := LocV new]>le, <[new := (t, vargs)]>h) 1
+    | GetEv: ∀ le h lhs recv name l t vs v,
+        expr_eval le recv = Some (LocV l) →
+        h !! l = Some (t, vs) →
+        vs !! name = Some v →
+        cmd_eval (le, h) (GetC lhs recv name) (<[lhs := v]>le, h) 1
+    | SetEv: ∀ le h recv fld rhs l v t vs vs',
+        expr_eval le recv = Some (LocV l) →
+        expr_eval le rhs = Some v →
+        h !! l = Some (t, vs) →
+        vs' = <[ fld := v ]>vs →
+        cmd_eval (le, h) (SetC recv fld rhs) (le, <[l := (t, vs')]> h) 0
+    | SeqEv: ∀ st1 st2 st3 fstc sndc n1 n2,
+        cmd_eval st1 fstc st2 n1 →
+        cmd_eval st2 sndc st3 n2 →
+        cmd_eval st1 (SeqC fstc sndc) st3 (n1 + n2)
+    | IfTrueEv: ∀ st1 st2 cond thn els n,
+        expr_eval st1.1 cond = Some (BoolV true) →
+        cmd_eval st1 thn st2 n →
+        cmd_eval st1 (IfC cond thn els) st2 n
+    | IfFalseEv: ∀ st1 st2 cond thn els n,
+        expr_eval st1.1 cond = Some (BoolV false) →
+        cmd_eval st1 els st2 n →
+        cmd_eval st1 (IfC cond thn els) st2 n
+    | CallEv: ∀ le h h' lhs recv l t vs name args vargs orig mdef
+        run_env run_env' ret n,
+        expr_eval le recv = Some (LocV l) →
+        map_args (expr_eval le) args = Some vargs →
+        h !! l = Some (t, vs) →
+        has_method name t orig mdef →
+        <["$this" := LocV l]>vargs = run_env →
+        cmd_eval (run_env, h) mdef.(methodbody) (run_env', h') n →
+        expr_eval run_env' mdef.(methodret) = Some ret →
+        cmd_eval (le, h) (CallC lhs recv name args) (<[lhs := ret]>le, h') (S n)
+    | CondTag1Ev n st1 st2 v t cmd :
+        (* tag in heap must <: requested tag to move forward *)
+        tag_match st1 v t →
+        cmd_eval st1 cmd st2 n →
+        cmd_eval st1 (CondTagC v t cmd) st2 n
+    | CondTag2Ev n st v t cmd :
+        ¬tag_match st v t →
+        cmd_eval st (CondTagC v t cmd) st n
 .
+
 End ProgDef.
 
 (* Hints and notations are local to the section. Re-exporting them *)
 Global Hint Constructors subtype : core.
 Global Hint Constructors has_field : core.
-Global Hint Constructors has_method : code.
+Global Hint Constructors has_method : core.
